@prefix : <https://saref.etsi.org/saref4auto/> .
@prefix owl: <http://www.w3.org/2002/07/owl#> .
@prefix rdf: <http://www.w3.org/1999/02/22-rdf-syntax-ns#> .
@prefix xml: <http://www.w3.org/XML/1998/namespace> .
@prefix xsd: <http://www.w3.org/2001/XMLSchema#> .
@prefix rdfs: <http://www.w3.org/2000/01/rdf-schema#> .
@base <https://saref.etsi.org/saref4auto/> .

<https://saref.etsi.org/saref4auto/> rdf:type owl:Ontology ;
                                      owl:versionIRI <https://saref.etsi.org/saref4auto/v1.1.1/> ;
                                      <http://purl.org/dc/terms/contributor> <https://scholar.google.com/citations?user=coCDIj8AAAAJ> ;
                                      <http://purl.org/dc/terms/creator> <http://netellany.fr/> ,
                                                                         <https://www.linkedin.com/in/lauradaniele> ;
                                      <http://purl.org/dc/terms/description> "This ontology extends the SAREF ontology for the automotive domain. This work has been developed in the context of the STF 566, which was established with the goal to create four SAREF extensions, one of them for the automotive domain."@en ;
                                      <http://purl.org/dc/terms/issued> "2020-07-27"^^xsd:date ;
                                      <http://purl.org/dc/terms/license> <https://forge.etsi.org/etsi-software-license> ;
                                      <http://purl.org/dc/terms/modified> "2021-07-26"^^xsd:date ;
                                      <http://purl.org/dc/terms/publisher> <https://www.etsi.org/> ;
                                      <http://purl.org/dc/terms/source> <https://saref.etsi.org/sources/saref4auto/> ;
                                      <http://purl.org/dc/terms/title> "SAREF extension for automotive"@en ;
                                      <http://purl.org/vocab/vann/preferredNamespacePrefix> "s4auto" ;
                                      <http://purl.org/vocab/vann/preferredNamespaceUri> "https://saref.etsi.org/saref4auto/" ;
                                      rdfs:seeAlso <https://www.etsi.org/deliver/etsi_ts/103400_103499/10341007/01.01.01_60/ts_10341007v010101p.pdf> ;
                                      owl:versionInfo "v1.1.1" .

#################################################################
#    Annotation properties
#################################################################

###  http://purl.org/dc/terms/contributor
<http://purl.org/dc/terms/contributor> rdf:type owl:AnnotationProperty .


###  http://purl.org/dc/terms/creator
<http://purl.org/dc/terms/creator> rdf:type owl:AnnotationProperty .


###  http://purl.org/dc/terms/description
<http://purl.org/dc/terms/description> rdf:type owl:AnnotationProperty .


###  http://purl.org/dc/terms/issued
<http://purl.org/dc/terms/issued> rdf:type owl:AnnotationProperty .


###  http://purl.org/dc/terms/license
<http://purl.org/dc/terms/license> rdf:type owl:AnnotationProperty .


###  http://purl.org/dc/terms/modified
<http://purl.org/dc/terms/modified> rdf:type owl:AnnotationProperty .


###  http://purl.org/dc/terms/publisher
<http://purl.org/dc/terms/publisher> rdf:type owl:AnnotationProperty .


###  http://purl.org/dc/terms/source
<http://purl.org/dc/terms/source> rdf:type owl:AnnotationProperty .


###  http://purl.org/dc/terms/title
<http://purl.org/dc/terms/title> rdf:type owl:AnnotationProperty .


###  http://purl.org/vocab/vann/preferredNamespacePrefix
<http://purl.org/vocab/vann/preferredNamespacePrefix> rdf:type owl:AnnotationProperty .


###  http://purl.org/vocab/vann/preferredNamespaceUri
<http://purl.org/vocab/vann/preferredNamespaceUri> rdf:type owl:AnnotationProperty .


#################################################################
#    Object Properties
#################################################################

###  http://www.opengis.net/ont/geosparql#hasGeometry
<http://www.opengis.net/ont/geosparql#hasGeometry> rdf:type owl:ObjectProperty ;
                                                   rdfs:domain <http://www.opengis.net/ont/geosparql#Feature> ;
                                                   rdfs:range <http://www.opengis.net/ont/geosparql#Geometry> ;
                                                   rdfs:comment "A spatial representation for a given feature." ;
                                                   rdfs:isDefinedBy <http://www.opengis.net/ont/geosparql> .


###  http://www.w3.org/2003/01/geo/wgs84_pos#location
<http://www.w3.org/2003/01/geo/wgs84_pos#location> rdf:type owl:ObjectProperty ;
                                                   rdfs:range <http://www.w3.org/2003/01/geo/wgs84_pos#SpatialThing> ;
                                                   rdfs:comment """The relation between something and the point, 
 or other geometrical thing in space, where it is.  For example, the realtionship between
 a radio tower and a Point with a given lat and long.
 Or a relationship between a park and its outline as a closed arc of points, or a road and
 its location as a arc (a sequence of points).
 Clearly in practice there will be limit to the accuracy of any such statement, but one would expect
 an accuracy appropriate for the size of the object and uses such as mapping .""" ;
                                                   rdfs:isDefinedBy "http://www.w3.org/2003/01/geo/wgs84_pos#" ;
                                                   rdfs:label "location"@en .


###  http://www.w3.org/2006/time#hasBeginning
<http://www.w3.org/2006/time#hasBeginning> rdf:type owl:ObjectProperty ;
                                           rdfs:domain <http://www.w3.org/2006/time#TemporalEntity> ;
                                           rdfs:range <http://www.w3.org/2006/time#Instant> ;
                                           rdfs:comment "Beginning of a temporal entity" ;
                                           rdfs:isDefinedBy "http://www.w3.org/2006/time" ;
                                           rdfs:label "hasBeginning"@en .


###  http://www.w3.org/2006/time#hasEnd
<http://www.w3.org/2006/time#hasEnd> rdf:type owl:ObjectProperty ;
                                     rdfs:domain <http://www.w3.org/2006/time#TemporalEntity> ;
                                     rdfs:range <http://www.w3.org/2006/time#Instant> ;
                                     rdfs:comment "End of a temporal entity." ;
                                     rdfs:isDefinedBy "http://www.w3.org/2006/time" ;
                                     rdfs:label "hasEnd"@en .


###  https://saref.etsi.org/core/consistsOf
<https://saref.etsi.org/core/consistsOf> rdf:type owl:ObjectProperty ;
                                         rdfs:comment "A relationship indicating a composite entity that consists of other entities (e.g., a temperature/humidity sensor that consists of a temperature sensor and a humidity sensor)"@en ;
                                         rdfs:isDefinedBy <https://saref.etsi.org/core> ;
                                         rdfs:label "consists of"@en .


###  https://saref.etsi.org/core/controlsProperty
<https://saref.etsi.org/core/controlsProperty> rdf:type owl:ObjectProperty ;
                                               rdfs:comment "A relationship specifying the property that can be controlled by a certain device"@en ;
                                               rdfs:isDefinedBy <https://saref.etsi.org/core/> ;
                                               rdfs:label "controls property"@en .


###  https://saref.etsi.org/core/hasProperty
<https://saref.etsi.org/core/hasProperty> rdf:type owl:ObjectProperty ;
                                          rdfs:domain <https://saref.etsi.org/core/FeatureOfInterest> ;
                                          rdfs:range <https://saref.etsi.org/core/Property> ;
                                          rdfs:comment "A relationship between a feature of interest and a property of that feature"@en ;
                                          rdfs:isDefinedBy <https://saref.etsi.org/core/> ;
                                          rdfs:label "controls property"@en .


###  https://saref.etsi.org/core/isControlledByDevice
<https://saref.etsi.org/core/isControlledByDevice> rdf:type owl:ObjectProperty ;
                                                   rdfs:comment "A relationship specifying the devices that can control a certain property"@en ;
                                                   rdfs:isDefinedBy <https://saref.etsi.org/core/> ;
                                                   rdfs:label "is controlled by device"@en .


###  https://saref.etsi.org/core/isMeasuredByDevice
<https://saref.etsi.org/core/isMeasuredByDevice> rdf:type owl:ObjectProperty ;
                                                 rdfs:comment "A relationship specifying the devices that can measure a certain property"@en ;
                                                 rdfs:isDefinedBy <https://saref.etsi.org/core/> ;
                                                 rdfs:label "is measured by device"@en .


###  https://saref.etsi.org/core/isMeasuredIn
<https://saref.etsi.org/core/isMeasuredIn> rdf:type owl:ObjectProperty ;
                                           rdfs:comment "A relationship identifying the unit of measure used for a certain entity."@en ;
                                           rdfs:isDefinedBy <https://saref.etsi.org/core/> ;
                                           rdfs:label "is measured in"@en .


###  https://saref.etsi.org/core/makesMeasurement
<https://saref.etsi.org/core/makesMeasurement> rdf:type owl:ObjectProperty ;
                                               owl:inverseOf <https://saref.etsi.org/core/measurementMadeBy> ;
                                               rdfs:comment "A relation between a device and the measurements it makes. Such measurement will link together the value of the measurement, its unit of measure and the property to which it relates."@en ;
                                               rdfs:isDefinedBy <https://saref.etsi.org/core/> ;
                                               rdfs:label "makes measurement"@en .


###  https://saref.etsi.org/core/measurementMadeBy
<https://saref.etsi.org/core/measurementMadeBy> rdf:type owl:ObjectProperty ;
                                                rdfs:comment "A relation between a measurement and the device that made it."@en ;
                                                rdfs:isDefinedBy <https://saref.etsi.org/core/> ;
                                                rdfs:label "measurementMadeBy"@en .


###  https://saref.etsi.org/core/measuresProperty
<https://saref.etsi.org/core/measuresProperty> rdf:type owl:ObjectProperty ;
                                               rdfs:domain <https://saref.etsi.org/core/Device> ;
                                               rdfs:range <https://saref.etsi.org/core/Property> ;
                                               rdfs:comment "A relationship specifying the property that can be measured by a certain device"@en ;
                                               rdfs:isDefinedBy <https://saref.etsi.org/core/> ;
                                               rdfs:label "measures property"@en .


###  https://saref.etsi.org/core/relatesToMeasurement
<https://saref.etsi.org/core/relatesToMeasurement> rdf:type owl:ObjectProperty ;
                                                   rdfs:comment "A relationship between a property and the measurements it relates to"@en ;
                                                   rdfs:isDefinedBy <https://saref.etsi.org/core/> ;
                                                   rdfs:label "relates to measurement"@en .


###  https://saref.etsi.org/core/relatesToProperty
<https://saref.etsi.org/core/relatesToProperty> rdf:type owl:ObjectProperty ;
                                                rdfs:comment "A relationship between a measurement and the property it relates to"@en ;
                                                rdfs:isDefinedBy <https://saref.etsi.org/core/> ;
                                                rdfs:label "relates to property"@en .


###  https://saref.etsi.org/saref4auto/consistsOfEntity
:consistsOfEntity rdf:type owl:ObjectProperty ;
                  rdfs:subPropertyOf <https://saref.etsi.org/core/consistsOf> ;
                  rdfs:comment "A relation to describe the entities that can compose the vehicle environment"@en ;
                  rdfs:label "consists Of Entity"@en .


###  https://saref.etsi.org/saref4auto/consistsOfEquipment
:consistsOfEquipment rdf:type owl:ObjectProperty ;
                     rdfs:subPropertyOf <https://saref.etsi.org/core/consistsOf> ;
                     rdfs:comment "A relation to describe the type of equipment that can compose the vehicle environment"@en ;
                     rdfs:label "consists of equipment"@en .


###  https://saref.etsi.org/saref4auto/consistsOfEvent
:consistsOfEvent rdf:type owl:ObjectProperty ;
                 rdfs:subPropertyOf <https://saref.etsi.org/core/consistsOf> ;
                 rdfs:comment "A relation to describe the events that can compose the vehicle environment"@en ;
                 rdfs:label "consists of event"@en .


###  https://saref.etsi.org/saref4auto/consistsOfObject
:consistsOfObject rdf:type owl:ObjectProperty ;
                  rdfs:subPropertyOf <https://saref.etsi.org/core/consistsOf> ;
                  rdfs:comment "A relation to describe the objects that can compose the vehicle environment"@en ;
                  rdfs:label "consists of object"@en .


###  https://saref.etsi.org/saref4auto/consistsOfUser
:consistsOfUser rdf:type owl:ObjectProperty ;
                rdfs:subPropertyOf <https://saref.etsi.org/core/consistsOf> ;
                rdfs:comment "A relation to describe the users that can compose the vehicle environment"@en ;
                rdfs:label "consists of user"@en .


###  https://saref.etsi.org/saref4auto/consistsOfVehicle
:consistsOfVehicle rdf:type owl:ObjectProperty ;
                   rdfs:subPropertyOf <https://saref.etsi.org/core/consistsOf> ;
                   rdfs:comment "A relation to decribe the vehicles that can compose the vehicle environment"@en ;
                   rdfs:label "consists of vehicle"@en .


###  https://saref.etsi.org/saref4auto/detectsPosition
:detectsPosition rdf:type owl:ObjectProperty ;
                 rdfs:comment "A relationship specifying the position (absolute or relative position) that can be detected by a certain device"@en ;
                 rdfs:label "detects position"@en .


###  https://saref.etsi.org/saref4auto/hasAbsolutePosition
:hasAbsolutePosition rdf:type owl:ObjectProperty ;
                     rdfs:subPropertyOf :hasPosition ;
                     rdfs:comment "A relation between an entity, e.g., a vehicle or road entity, and AbsolutePosition to represent its absolute position"@en ;
                     rdfs:label "hasAbsolutePosition"@en .


###  https://saref.etsi.org/saref4auto/hasAutomationLevel
:hasAutomationLevel rdf:type owl:ObjectProperty ;
                    rdfs:comment """A relation to define the level of automation of a singular vehicle. According to SAE J3016, there are five levels of automation:
- Level 0: No Driving Automation.
- Level 1: Driver assistance.
- Level 2: Partial driving automation.
- Level 3: Conditional driving automation.
- Level 4: High driving automation.
- Level 5: Full Driving automation.
."""@en ;
                    rdfs:label "hasAutomationLevel"@en .


###  https://saref.etsi.org/saref4auto/hasBrakeCapacity
:hasBrakeCapacity rdf:type owl:ObjectProperty ;
                  rdfs:range :BrakeCapacity ;
                  rdfs:comment "A relation to express that the vehicle has the capacity to reduce its speed (by action on the brake pedal or an autonomous actuator)"@en ;
                  rdfs:label "hasBrakeCapacity"@en .


###  https://saref.etsi.org/saref4auto/hasConfidence
:hasConfidence rdf:type owl:ObjectProperty ;
               owl:inverseOf :isConfidenceOf ;
               rdfs:range :Confidence ;
               rdfs:comment "A relation between an estimated measurement (saref:Measurement class) and its confidence (s4auto:Confidence)"@en ;
               rdfs:label "hasConfidence"@en .


###  https://saref.etsi.org/saref4auto/hasConfidenceUnitOfMeasure
:hasConfidenceUnitOfMeasure rdf:type owl:ObjectProperty ;
                            rdfs:comment "A relation that allows to specify the unit of measure associated with a certain confidence"@en ;
                            rdfs:label "has confidence unit of measure"@en .


###  https://saref.etsi.org/saref4auto/hasDestination
:hasDestination rdf:type owl:ObjectProperty ;
                rdfs:comment "A relation that defines the destination of an automotive object. For example, in a platoon, the current platoon leader defines the platoon destination. Following vehicles will share (partially) the route of the leader and can, therefore, have different final destinations." ;
                rdfs:label "hasDestination"@en .


###  https://saref.etsi.org/saref4auto/hasDestinationAddress
:hasDestinationAddress rdf:type owl:ObjectProperty ;
                       rdfs:subPropertyOf :hasDestination ;
                       rdfs:comment "A relation to express the destination of a vehicle in terms of an Address"@en ;
                       rdfs:label "hasDestinationAddress"@en .


###  https://saref.etsi.org/saref4auto/hasDestinationEndPoint
:hasDestinationEndPoint rdf:type owl:ObjectProperty ;
                        rdfs:subPropertyOf :hasDestination ;
                        rdfs:comment "A relation to express the destination of a vehicle, a platoon or a route in terms of an end point with latitude and longitude"@en ;
                        rdfs:label "hasDestinationEndPoint"@en .


###  https://saref.etsi.org/saref4auto/hasEnvironment
:hasEnvironment rdf:type owl:ObjectProperty ;
                rdfs:comment "A relation that allows to describe the environment of a vehicle"@en ;
                rdfs:label "hasEnvironment"@en .


###  https://saref.etsi.org/saref4auto/hasEstimatedRendezvousLocation
:hasEstimatedRendezvousLocation rdf:type owl:ObjectProperty ;
                                rdfs:range :RendezvousLocation ;
                                rdfs:comment "A relation to express that, during the forming state, a vehicle member of a platoon is given an estimated rendezvous location for joining the platoon. It is expressed in global coordinates (lat, long, alt), e.g. according to WGS 84." ;
                                rdfs:label "hasEstimatedRendezvousLocation"@en .


###  https://saref.etsi.org/saref4auto/hasHeight
:hasHeight rdf:type owl:ObjectProperty ;
           rdfs:subPropertyOf <https://saref.etsi.org/core/hasProperty> ;
           rdfs:comment "A relation to express the height of an entity, e.g., a vehicle or an entity in the vehicle environment"@en ;
           rdfs:label "hasHeight"@en .


###  https://saref.etsi.org/saref4auto/hasIdentifier
:hasIdentifier rdf:type owl:ObjectProperty ;
               rdfs:range :Identifier ;
               rdfs:comment "A relation between an entity and its identifier (s4auto:Identifier) which is used to identify 1) a vehicle (station) during data exchange with other devices/stations 2) a platoon during data exchange with other devices/stations, 3) a parking spot within a parking area during data exchange with other devices/stations. In all cases, this identifier may be a pseudonym. It may change over space and/or over time."@en ;
               rdfs:label "hasIdentifier"@en .


###  https://saref.etsi.org/saref4auto/hasLength
:hasLength rdf:type owl:ObjectProperty ;
           rdfs:subPropertyOf <https://saref.etsi.org/core/hasProperty> ;
           rdfs:comment "A relation to express the length of an entity, e.g., a vehicle or an entity in the vehicle environment or a platoon (Length of the platoon is the sum of all vehicles' length + inter-vehicle distance)"@en ;
           rdfs:label "hasLength"@en .


###  https://saref.etsi.org/saref4auto/hasMember
:hasMember rdf:type owl:ObjectProperty ;
           owl:inverseOf :isMemberOf ;
           rdfs:comment "A general relationship to express that an entity can have members"@en ;
           rdfs:label "hasMember"@en .


###  https://saref.etsi.org/saref4auto/hasMovement
:hasMovement rdf:type owl:ObjectProperty ;
             rdfs:subPropertyOf <https://saref.etsi.org/core/hasProperty> ;
             rdfs:comment "A relation to express the movement of an entity in the vehicle environment."@en ;
             rdfs:label "hasMovement"@en .


###  https://saref.etsi.org/saref4auto/hasOpeningTimeAvailability
:hasOpeningTimeAvailability rdf:type owl:ObjectProperty ;
                            rdfs:comment "A relation to express the opening time of parking spot"@en ;
                            rdfs:label "hasOpeningTimeAvailability"@en .


###  https://saref.etsi.org/saref4auto/hasOrigin
:hasOrigin rdf:type owl:ObjectProperty ;
           rdfs:comment "A relation to express the origin of an entity (e.g., a vehicle or a route)  in terms of a StartPoint"@en ;
           rdfs:label "hasOrigin"@en .


###  https://saref.etsi.org/saref4auto/hasParkingSpotState
:hasParkingSpotState rdf:type owl:ObjectProperty ;
                     rdfs:subPropertyOf :hasState ;
                     rdfs:comment "A relation to express the state of a parking spot"@en ;
                     rdfs:label "hasParkingSpotState"@en .


###  https://saref.etsi.org/saref4auto/hasParkingVehicleState
:hasParkingVehicleState rdf:type owl:ObjectProperty ;
                        rdfs:subPropertyOf :hasState ;
                        rdfs:comment "A relation to express the state of a vehicle that is parking"@en ;
                        rdfs:label "hasParkingVehicleState"@en .


###  https://saref.etsi.org/saref4auto/hasPerceptionState
:hasPerceptionState rdf:type owl:ObjectProperty ;
                    rdfs:subPropertyOf :hasState ;
                    rdfs:comment "A relation to express the state of a vehicle related to its environment"@en ;
                    rdfs:label "hasPerceptionState"@en .


###  https://saref.etsi.org/saref4auto/hasPlatoonMember
:hasPlatoonMember rdf:type owl:ObjectProperty ;
                  rdfs:subPropertyOf :hasMember ;
                  rdfs:comment "A relation to express that a platoon can have vehicles as its members"@en ;
                  rdfs:label "hasPlatoonMember"@en .


###  https://saref.etsi.org/saref4auto/hasPlatoonPosition
:hasPlatoonPosition rdf:type owl:ObjectProperty ;
                    rdfs:subPropertyOf :hasPosition ;
                    rdfs:comment "A relatiA relation to express that a vehicle member of a platoon has a platoon position that is defined as the index of the vehicle in the platoon starting from zero (leader) up to N (trailing vehicle)"@en ;
                    rdfs:label "hasPlatoonPosition"@en .


###  https://saref.etsi.org/saref4auto/hasPlatoonRole
:hasPlatoonRole rdf:type owl:ObjectProperty ;
                rdfs:subPropertyOf :hasRole ;
                rdfs:comment "A relation to specify that in a platoon a vehicle can assume roles such as: unknown, leader, follower, ready-for-leading, trailing, etc."@en ;
                rdfs:label "hasPlatoonRole"@en .


###  https://saref.etsi.org/saref4auto/hasPlatoonState
:hasPlatoonState rdf:type owl:ObjectProperty ;
                 rdfs:subPropertyOf :hasState ;
                 rdfs:comment "A relation to express the state of a platoon"@en ;
                 rdfs:label "hasPlatoonState"@en .


###  https://saref.etsi.org/saref4auto/hasPlatoonVehicleState
:hasPlatoonVehicleState rdf:type owl:ObjectProperty ;
                        rdfs:subPropertyOf :hasState ;
                        rdfs:comment "A relation to express the state of a vehicle in a platoon"@en ;
                        rdfs:label "hasPlatoonVehicleState"@en .


###  https://saref.etsi.org/saref4auto/hasPosition
:hasPosition rdf:type owl:ObjectProperty ;
             rdfs:range :RelativePosition ;
             rdfs:comment "A relation to define the position of an entity"@en ;
             rdfs:label "has position"@en .


###  https://saref.etsi.org/saref4auto/hasRelativePosition
:hasRelativePosition rdf:type owl:ObjectProperty ;
                     rdfs:subPropertyOf :hasPosition ;
                     rdfs:comment "A relation between an entity, e.g., a vehicle or road entity, and RelativePosition to represent its relative position (e.g., a car is x,y,z in front of another car)"@en ;
                     rdfs:label "hasPlatoonPosition"@en .


###  https://saref.etsi.org/saref4auto/hasRoadTopologyPosition
:hasRoadTopologyPosition rdf:type owl:ObjectProperty ;
                         rdfs:subPropertyOf :hasPosition ;
                         rdfs:comment "A relation between Vehicle and RoadTopologyPosition to represent the road topology position of a vehicle"@en ;
                         rdfs:label "hasRoadTopologyPosition"@en .


###  https://saref.etsi.org/saref4auto/hasRole
:hasRole rdf:type owl:ObjectProperty ;
         rdfs:range :Role ;
         rdfs:comment "A general relation to express that an entity can have a role"@en ;
         rdfs:label "hasRole"@en .


###  https://saref.etsi.org/saref4auto/hasRoute
:hasRoute rdf:type owl:ObjectProperty ;
          rdfs:comment "A relation to express the route of an entity, e.g., a vehicle or a platoon"@en ;
          rdfs:label "hasRoute"@en .


###  https://saref.etsi.org/saref4auto/hasShape
:hasShape rdf:type owl:ObjectProperty ;
          rdfs:subPropertyOf <https://saref.etsi.org/core/hasProperty> ;
          rdfs:comment "A relation to express the shape of an entity in the vehicle environment."@en ;
          rdfs:label "hasShape"@en .


###  https://saref.etsi.org/saref4auto/hasSize
:hasSize rdf:type owl:ObjectProperty ;
         rdfs:subPropertyOf <https://saref.etsi.org/core/hasProperty> ;
         rdfs:comment "A relation to express that a platoon has a size. This size is defined as 1) the total number of vehicles currently in the platoon; or 2) Length of the platoon (sum of all vehicles' length + inter-vehicle distance) via s4auto:hasLength property"@en ;
         rdfs:label "hasSize"@en .


###  https://saref.etsi.org/saref4auto/hasState
:hasState rdf:type owl:ObjectProperty ;
          rdfs:comment "An hasState relation to connect to a certain state. The saref:hasState property could not be reused because it has domain saref:Device, but a s4auto:Platoon or s4auto:Vehicle are not devices. Therefore, a new s4auto:hasState property with subroperties has been created."@en ;
          rdfs:label "hasState"@en .


###  https://saref.etsi.org/saref4auto/hasVehicleEnvironmentMember
:hasVehicleEnvironmentMember rdf:type owl:ObjectProperty ;
                             rdfs:subPropertyOf :hasMember ;
                             rdfs:comment "A relation to express that a vehicle can have members in its environment"@en ;
                             rdfs:label "hasVehicleEnvironmentMember"@en .


###  https://saref.etsi.org/saref4auto/hasVehicleRole
:hasVehicleRole rdf:type owl:ObjectProperty ;
                rdfs:subPropertyOf :hasRole ;
                rdfs:comment "A relation between Vehicle and VehicleRole classes, to express the role the vehicle plays in traffic. If not specified, it is assumed that it takes a default value. Otherwise, possible values to be specified are: publicTransport, specialTransport, dangerousGoods, roadWork, rescue, emergency, safetyCar, agriculture, commercial, military, roadOperator, taxi (see ETSI TR 103 508)."@en ;
                rdfs:label "hasVehicleRole"@en .


###  https://saref.etsi.org/saref4auto/hasWidth
:hasWidth rdf:type owl:ObjectProperty ;
          rdfs:subPropertyOf <https://saref.etsi.org/core/hasProperty> ;
          rdfs:comment "A relation to express the width of an entity, e.g., a vehicle or an entity in the vehicle environment"@en ;
          rdfs:label "hasWidth"@en .


###  https://saref.etsi.org/saref4auto/isCollectionOf
:isCollectionOf rdf:type owl:ObjectProperty ;
                rdfs:comment "A relation to express the intermediate destination of a route (e.g., of a vehicle or a platoon) in terms of RoutePoint"@en ;
                rdfs:label "isCollectionOf"@en .


###  https://saref.etsi.org/saref4auto/isConfidenceOf
:isConfidenceOf rdf:type owl:ObjectProperty ;
                rdfs:comment "A relation between the confidence (s4auto:Confidence class) of an estimated measurement and this measurement (saref:Measurement class)"@en ;
                rdfs:label "isConfidenceOf"@en .


###  https://saref.etsi.org/saref4auto/isMemberOf
:isMemberOf rdf:type owl:ObjectProperty ;
            rdfs:comment "A general relationship to express that an entity is a member of another entity"@en ;
            rdfs:label "isMemberOf"@en .


###  https://saref.etsi.org/saref4auto/isMemberOfPlatoon
:isMemberOfPlatoon rdf:type owl:ObjectProperty ;
                   rdfs:subPropertyOf :isMemberOf ;
                   rdfs:comment "A relation to express that a vehicle can be member of  a platoon"@en ;
                   rdfs:label "isMemberOfPlatoon"@en .


###  https://saref.etsi.org/saref4auto/isMemberOfVehicleEnvironment
:isMemberOfVehicleEnvironment rdf:type owl:ObjectProperty ;
                              rdfs:subPropertyOf :isMemberOf ;
                              rdfs:comment "A relation to express that an entity, e.g., a vehicle, can be member of  another vehicle's environment"@en ;
                              rdfs:label "isMemberOfVehicleEnvironment"@en .


###  https://saref.etsi.org/saref4auto/usesMeasurement
:usesMeasurement rdf:type owl:ObjectProperty ;
                 rdfs:comment "A relation to express that a device can use different types of measurements, such as speed, position of detected road objects (e.g., bicycles, vehicles). This applies in particular to the ElectronicControlUnit and TrafficLightController classes."@en ;
                 rdfs:label "usesMeasurement"@en .


###  https://saref.etsi.org/saref4syst/hasSubSystem
<https://saref.etsi.org/saref4syst/hasSubSystem> rdf:type owl:ObjectProperty ;
                                                 owl:inverseOf <https://saref.etsi.org/saref4syst/subSystemOf> ;
                                                 rdfs:comment "In SAREF4AUTO, a  relation to express that the vehicle has a subsystem called ‘ElectronicControlUnit' (ECU) that provides measurements about relevant properties, such as speed, acceleration, position, etc."@en ,
                                                              "Links a system to one of its sub systems"@en ;
                                                 rdfs:isDefinedBy <https://saref.etsi.org/saref4syst/> ;
                                                 rdfs:label "hasSubSystem"@en .


###  https://saref.etsi.org/saref4syst/subSystemOf
<https://saref.etsi.org/saref4syst/subSystemOf> rdf:type owl:ObjectProperty ;
                                                rdfs:comment "In SAREF4AUTO, a relation to express that the the ElectronicControlUnit (ECU) is a subsystem of the vehicle."@en ,
                                                             "Links a system to its super system. Properties of subsystems somehow contribute to the properties of the super system. The exact meaning of \"contribute is defined by sub properties of s4syst:subSystemOf. Property s4syst:subSystemOf is transitive."@en ;
                                                rdfs:isDefinedBy <https://saref.etsi.org/saref4syst/> ;
                                                rdfs:label "subSystemOf"@en .


#################################################################
#    Data properties
#################################################################

###  http://www.w3.org/2003/01/geo/wgs84_pos#alt
<http://www.w3.org/2003/01/geo/wgs84_pos#alt> rdf:type owl:DatatypeProperty ;
                                              rdfs:domain <http://www.w3.org/2003/01/geo/wgs84_pos#SpatialThing> ;
                                              rdfs:comment """The WGS84 altitude of a SpatialThing (decimal meters 
above the local reference ellipsoid).""" ;
                                              rdfs:isDefinedBy "http://www.w3.org/2003/01/geo/wgs84_pos" ;
                                              rdfs:label "altitude" .


###  http://www.w3.org/2003/01/geo/wgs84_pos#lat
<http://www.w3.org/2003/01/geo/wgs84_pos#lat> rdf:type owl:DatatypeProperty ;
                                              rdfs:domain <http://www.w3.org/2003/01/geo/wgs84_pos#SpatialThing> ;
                                              rdfs:comment "The WGS84 latitude of a SpatialThing (decimal degrees)." ;
                                              rdfs:isDefinedBy "http://www.w3.org/2003/01/geo/wgs84_pos" ;
                                              rdfs:label "latitude" .


###  http://www.w3.org/2003/01/geo/wgs84_pos#long
<http://www.w3.org/2003/01/geo/wgs84_pos#long> rdf:type owl:DatatypeProperty ;
                                               rdfs:domain <http://www.w3.org/2003/01/geo/wgs84_pos#SpatialThing> ;
                                               rdfs:comment "The WGS84 longitude of a SpatialThing (decimal degrees)." ;
                                               rdfs:isDefinedBy "http://www.w3.org/2003/01/geo/wgs84_pos" ;
                                               rdfs:label "longitude" .


###  http://www.w3.org/2006/time#inXSDDateTimeStamp
<http://www.w3.org/2006/time#inXSDDateTimeStamp> rdf:type owl:DatatypeProperty ;
                                                 rdfs:domain <http://www.w3.org/2006/time#Instant> ;
                                                 rdfs:range xsd:dateTimeStamp ;
                                                 rdfs:comment "Position of an instant, expressed using xsd:dateTimeStamp" ;
                                                 rdfs:isDefinedBy "http://www.w3.org/2006/time" ;
                                                 rdfs:label "inXSDDateTimeStamp"@en .


###  https://saref.etsi.org/core/hasTimestamp
<https://saref.etsi.org/core/hasTimestamp> rdf:type owl:DatatypeProperty ;
                                           rdfs:comment "A relationship stating the timestamp of an entity (e.g. a measurement)."@en ;
                                           rdfs:isDefinedBy <https://saref.etsi.org/core> ;
                                           rdfs:label "has timestamp"@en .


###  https://saref.etsi.org/core/hasValue
<https://saref.etsi.org/core/hasValue> rdf:type owl:DatatypeProperty ;
                                       rdfs:comment <https://saref.etsi.org/core> ,
                                                    "A relationship defining the value of a certain property, e.g., energy or power. Note that, even if numeric values are expected to enable reasoning, measurement values could use other datatypes."@en ;
                                       rdfs:label "has value"@en .


###  https://saref.etsi.org/saref4auto/hasConfidenceValue
:hasConfidenceValue rdf:type owl:DatatypeProperty ;
                    rdfs:comment "A relation between the confidence (s4auto:Confidence) and its value, which can be a discrete value (+/- 5 cm/s) or a level (e.g. 95 %)"@en ;
                    rdfs:label "hasConfidenceValue"@en .


###  https://saref.etsi.org/saref4auto/hasCoordinateX
:hasCoordinateX rdf:type owl:DatatypeProperty ;
                rdfs:comment "A relation to define the X coordinate of a relative position"@en ;
                rdfs:label "hasCoordinateX"@en .


###  https://saref.etsi.org/saref4auto/hasCoordinateY
:hasCoordinateY rdf:type owl:DatatypeProperty ;
                rdfs:comment "A relation to define the Y coordinate of a relative position"@en ;
                rdfs:label "hasCoordinateY"@en .


###  https://saref.etsi.org/saref4auto/hasCoordinateZ
:hasCoordinateZ rdf:type owl:DatatypeProperty ;
                rdfs:comment "A relation to define the Z coordinate of a relative position"@en ;
                rdfs:label "hasCoordinateY"@en .


###  https://saref.etsi.org/saref4auto/hasDescriptionName
:hasDescriptionName rdf:type owl:DatatypeProperty ;
                    rdfs:comment "A relation to define that a parking spot can have a description name"@en ;
                    rdfs:label "hasDescriptionName"@en .


###  https://saref.etsi.org/saref4auto/hasEstimatedJoiningTime
:hasEstimatedJoiningTime rdf:type owl:DatatypeProperty ;
                         rdfs:range xsd:dateTime ;
                         rdfs:comment "A relation to express that, during the forming state, a vehicle member of a platoon is given an estimated time for joining" ;
                         rdfs:label "hasEstimatedJoiningTime"@en .


###  https://saref.etsi.org/saref4auto/hasIDValue
:hasIDValue rdf:type owl:DatatypeProperty ;
            rdfs:comment "A relationship to define the value of an indentifier"@en ;
            rdfs:label "hasIDValue"@en .


###  https://saref.etsi.org/saref4auto/hasMaxSize
:hasMaxSize rdf:type owl:DatatypeProperty ;
            rdfs:comment "A relation to express the max size of a platoon. Note that it is defined as a datatype property as this is a fixed/static value of the platoon that does not change over time. In contrast, the current size of the platoon is actually a measurement that may change over time and it is therefore defined as an object property (see s4auto:hasSize)."@en ;
            rdfs:label "hasMaxSize"@en .


###  https://saref.etsi.org/saref4auto/hasPlatoonIndex
:hasPlatoonIndex rdf:type owl:DatatypeProperty ;
                 rdfs:range xsd:int ;
                 rdfs:comment "A relation to express the index of the vehicle in the platoon starting from zero (leader) up to N (trailing vehicle)"@en ;
                 rdfs:label "hasPlatoonIndex"@en .


#################################################################
#    Classes
#################################################################

###  http://www.opengis.net/ont/geosparql#Feature
<http://www.opengis.net/ont/geosparql#Feature> rdf:type owl:Class ;
                                               rdfs:subClassOf <http://www.opengis.net/ont/geosparql#SpatialObject> ;
                                               owl:disjointWith <http://www.opengis.net/ont/geosparql#Geometry> ;
                                               rdfs:comment """This class represents the top-level feature type. This class is 
      equivalent to GFI_Feature defined in ISO 19156:2011, and it is 
      superclass of all feature types.""" ;
                                               rdfs:isDefinedBy <http://www.opengis.net/ont/geosparql> ;
                                               rdfs:label "Feature"@en .


###  http://www.opengis.net/ont/geosparql#Geometry
<http://www.opengis.net/ont/geosparql#Geometry> rdf:type owl:Class ;
                                                rdfs:subClassOf <http://www.opengis.net/ont/geosparql#SpatialObject> ;
                                                rdfs:comment """The class represents the top-level geometry type. This class is 
      equivalent to the UML class GM_Object defined in ISO 19107, and 
      it is superclass of all geometry types.""" ;
                                                rdfs:isDefinedBy <http://www.opengis.net/ont/geosparql> ;
                                                rdfs:label "Geometry"@en .


###  http://www.opengis.net/ont/geosparql#SpatialObject
<http://www.opengis.net/ont/geosparql#SpatialObject> rdf:type owl:Class ;
                                                     rdfs:comment """The class spatial-object represents everything that can have 
      a spatial representation. It is superclass of feature and geometry.""" ;
                                                     rdfs:isDefinedBy <http://www.opengis.net/ont/geosparql> ;
                                                     rdfs:label "SpatialObject"@en .


###  http://www.w3.org/2003/01/geo/wgs84_pos#Point
<http://www.w3.org/2003/01/geo/wgs84_pos#Point> rdf:type owl:Class ;
                                                rdfs:subClassOf <http://www.w3.org/2003/01/geo/wgs84_pos#SpatialThing> ;
                                                rdfs:comment "A point, typically described using a coordinate system relative to Earth, such as WGS84." ,
                                                             """Uniquely identified by lat/long/alt. i.e.

spaciallyIntersects(P1, P2) :- lat(P1, LAT), long(P1, LONG), alt(P1, ALT),
  lat(P2, LAT), long(P2, LONG), alt(P2, ALT).

sameThing(P1, P2) :- type(P1, Point), type(P2, Point), spaciallyIntersects(P1, P2).""" ;
                                                rdfs:isDefinedBy "http://www.w3.org/2003/01/geo/wgs84_pos#" ;
                                                rdfs:label "Point"@en .


###  http://www.w3.org/2003/01/geo/wgs84_pos#SpatialThing
<http://www.w3.org/2003/01/geo/wgs84_pos#SpatialThing> rdf:type owl:Class ;
                                                       rdfs:comment """Anything with spatial extent, i.e. size, shape, or position.
 e.g. people, places, bowling balls, as well as abstract areas like cubes.""" ;
                                                       rdfs:isDefinedBy "http://www.w3.org/2003/01/geo/wgs84_pos#" ;
                                                       rdfs:label "Spatial Thing"@en .


###  http://www.w3.org/2006/time#Instant
<http://www.w3.org/2006/time#Instant> rdf:type owl:Class ;
                                      rdfs:subClassOf <http://www.w3.org/2006/time#TemporalEntity> ;
                                      rdfs:comment "A temporal entity with zero extent or duration" ;
                                      rdfs:isDefinedBy "http://www.w3.org/2006/time" ;
                                      rdfs:label "Instant"@en .


###  http://www.w3.org/2006/time#Interval
<http://www.w3.org/2006/time#Interval> rdf:type owl:Class ;
                                       rdfs:subClassOf <http://www.w3.org/2006/time#TemporalEntity> ;
                                       rdfs:comment "A temporal entity with an extent or duration" ;
                                       rdfs:isDefinedBy "http://www.w3.org/2006/time" ;
                                       rdfs:label "Interval"@en .


###  http://www.w3.org/2006/time#TemporalEntity
<http://www.w3.org/2006/time#TemporalEntity> rdf:type owl:Class ;
                                             rdfs:comment "A temporal interval or instant." ;
                                             rdfs:isDefinedBy "http://www.w3.org/2006/time" ;
                                             rdfs:label "TemporaryEntity"@en .


###  https://saref.etsi.org/core/Actuator
<https://saref.etsi.org/core/Actuator> rdf:type owl:Class ;
                                       rdfs:subClassOf <https://saref.etsi.org/core/Device> ;
                                       rdfs:comment "A device responsible for moving or controlling a mechanism or system."@en ;
                                       rdfs:isDefinedBy <https://saref.etsi.org/core> ;
                                       rdfs:label "Actuator"@en .


###  https://saref.etsi.org/core/Device
<https://saref.etsi.org/core/Device> rdf:type owl:Class ;
                                     rdfs:subClassOf [ rdf:type owl:Restriction ;
                                                       owl:onProperty <https://saref.etsi.org/core/controlsProperty> ;
                                                       owl:allValuesFrom <https://saref.etsi.org/core/Property>
                                                     ] ,
                                                     [ rdf:type owl:Restriction ;
                                                       owl:onProperty <https://saref.etsi.org/core/makesMeasurement> ;
                                                       owl:allValuesFrom <https://saref.etsi.org/core/Measurement>
                                                     ] ,
                                                     [ rdf:type owl:Restriction ;
                                                       owl:onProperty <https://saref.etsi.org/core/measuresProperty> ;
                                                       owl:allValuesFrom <https://saref.etsi.org/core/Property>
                                                     ] ;
                                     rdfs:comment "A tangible object designed to accomplish a particular task in households, common public buildings or offices. In order to accomplish this task, the device performs one or more functions. For example, a washing machine is designed to wash (task) and to accomplish this task it performs a start and stop function. Devices can be structured in categories (subclasses) that reflect the different domain in which a device is used, e.g., smart appliances domain (subclass FunctionRelated) vs. building domain (subclass BuildingRelated) vs. smart grid domain (subclass EnergyRelated). New categories can be defined,if needed, to reflect other differences, for example different points of view, such as the point of view of the device's user vs. the point of view of the device's manufacturer. We propose a list of devices that are relevant for the purpose of SAREF, but this list can be extended."@en ;
                                     rdfs:isDefinedBy <https://saref.etsi.org/core/> ;
                                     rdfs:label "Device"@en .


###  https://saref.etsi.org/core/FeatureOfInterest
<https://saref.etsi.org/core/FeatureOfInterest> rdf:type owl:Class ;
                                                rdfs:subClassOf [ rdf:type owl:Restriction ;
                                                                  owl:onProperty :hasIdentifier ;
                                                                  owl:someValuesFrom :Identifier
                                                                ] ,
                                                                [ rdf:type owl:Restriction ;
                                                                  owl:onProperty <https://saref.etsi.org/core/hasProperty> ;
                                                                  owl:allValuesFrom <https://saref.etsi.org/core/Property>
                                                                ] ;
                                                rdfs:comment "A feature of interest represents any real world entity from which a property is measured."@en ;
                                                rdfs:isDefinedBy <https://saref.etsi.org/core/> ;
                                                rdfs:label "FeatureOfInterest"@en .


###  https://saref.etsi.org/core/Measurement
<https://saref.etsi.org/core/Measurement> rdf:type owl:Class ;
                                          rdfs:subClassOf [ rdf:type owl:Restriction ;
                                                            owl:onProperty <https://saref.etsi.org/core/measurementMadeBy> ;
                                                            owl:someValuesFrom <https://saref.etsi.org/core/Device>
                                                          ] ,
                                                          [ rdf:type owl:Restriction ;
                                                            owl:onProperty :hasConfidence ;
                                                            owl:someValuesFrom :Confidence
                                                          ] ,
                                                          [ rdf:type owl:Restriction ;
                                                            owl:onProperty <https://saref.etsi.org/core/isMeasuredIn> ;
                                                            owl:allValuesFrom <https://saref.etsi.org/core/UnitOfMeasure>
                                                          ] ,
                                                          [ rdf:type owl:Restriction ;
                                                            owl:onProperty <https://saref.etsi.org/core/relatesToProperty> ;
                                                            owl:allValuesFrom <https://saref.etsi.org/core/Property>
                                                          ] ,
                                                          [ rdf:type owl:Restriction ;
                                                            owl:onProperty <https://saref.etsi.org/core/isMeasuredIn> ;
                                                            owl:qualifiedCardinality "1"^^xsd:nonNegativeInteger ;
                                                            owl:onClass <https://saref.etsi.org/core/UnitOfMeasure>
                                                          ] ,
                                                          [ rdf:type owl:Restriction ;
                                                            owl:onProperty <https://saref.etsi.org/core/relatesToProperty> ;
                                                            owl:qualifiedCardinality "1"^^xsd:nonNegativeInteger ;
                                                            owl:onClass <https://saref.etsi.org/core/Property>
                                                          ] ,
                                                          [ rdf:type owl:Restriction ;
                                                            owl:onProperty <https://saref.etsi.org/core/hasTimestamp> ;
                                                            owl:allValuesFrom xsd:dateTime
                                                          ] ,
                                                          [ rdf:type owl:Restriction ;
                                                            owl:onProperty <https://saref.etsi.org/core/hasValue> ;
                                                            owl:qualifiedCardinality "1"^^xsd:nonNegativeInteger ;
                                                            owl:onDataRange xsd:float
                                                          ] ;
                                          rdfs:comment "Represents the measured value made over a property. It is also linked to the unit of measure in which the value is expressed and the timestamp of the measurement."@en ;
                                          rdfs:isDefinedBy <https://saref.etsi.org/core/> ;
                                          rdfs:label "Measurement"@en .


###  https://saref.etsi.org/core/Property
<https://saref.etsi.org/core/Property> rdf:type owl:Class ;
                                       rdfs:subClassOf [ rdf:type owl:Restriction ;
                                                         owl:onProperty <https://saref.etsi.org/core/isControlledByDevice> ;
                                                         owl:allValuesFrom <https://saref.etsi.org/core/Device>
                                                       ] ,
                                                       [ rdf:type owl:Restriction ;
                                                         owl:onProperty <https://saref.etsi.org/core/isMeasuredByDevice> ;
                                                         owl:allValuesFrom <https://saref.etsi.org/core/Device>
                                                       ] ,
                                                       [ rdf:type owl:Restriction ;
                                                         owl:onProperty <https://saref.etsi.org/core/relatesToMeasurement> ;
                                                         owl:allValuesFrom <https://saref.etsi.org/core/Measurement>
                                                       ] ;
                                       rdfs:comment "Anything that can be sensed, measured or controlled by a device (measured by a sensor, controlled by an actuator) ."@en ;
                                       rdfs:isDefinedBy <https://saref.etsi.org/core> ;
                                       rdfs:label "Property"@en .


###  https://saref.etsi.org/core/Sensor
<https://saref.etsi.org/core/Sensor> rdf:type owl:Class ;
                                     rdfs:subClassOf <https://saref.etsi.org/core/Device> ;
                                     rdfs:comment "A device that detects and responds to events or changes in the physical environment such as light, motion, or temperature changes. A device that has category saref:Sensor and performs a saref:SensingFunction."@en ;
                                     rdfs:isDefinedBy <https://saref.etsi.org/core> ;
                                     rdfs:label "Sensor"@en .


###  https://saref.etsi.org/core/State
<https://saref.etsi.org/core/State> rdf:type owl:Class ;
                                    rdfs:comment "The state in which a device can be found, e.g, ON/OFF/STANDBY, or ONLINE/OFFLINE. We propose here a list of states that are relevant for the purpose of SAREF, but this list can be extended."@en ;
                                    rdfs:isDefinedBy <https://saref.etsi.org/core> ;
                                    rdfs:label "State"@en .


###  https://saref.etsi.org/core/UnitOfMeasure
<https://saref.etsi.org/core/UnitOfMeasure> rdf:type owl:Class ;
                                            rdfs:comment "The unit of measure is a standard for measurement of a quantity, such as a Property. For example, Power is a property and Watt is a unit of power that represents a definite predetermined power: when we say 10 Watt, we actually mean 10 times the definite predetermined power called \"watt\". Our definition is based on the definition of unit of measure in the Ontology of units of Measure (OM). We propose here a list of some units of measure that are relevant for the purpose of SAREF, but this list can be extended, also using some other ontologies rather than the Ontology of units of Measure (OM)."@en ;
                                            rdfs:isDefinedBy <https://saref.etsi.org/core/> ;
                                            rdfs:label "UnitOfMeasure"@en .


###  https://saref.etsi.org/saref4auto/AbsolutePosition
:AbsolutePosition rdf:type owl:Class ;
                  rdfs:subClassOf :Point ,
                                  :Position ,
                                  [ rdf:type owl:Restriction ;
                                    owl:onProperty <http://www.w3.org/2003/01/geo/wgs84_pos#alt> ;
                                    owl:someValuesFrom xsd:float
                                  ] ,
                                  [ rdf:type owl:Restriction ;
                                    owl:onProperty <http://www.w3.org/2003/01/geo/wgs84_pos#lat> ;
                                    owl:someValuesFrom xsd:float
                                  ] ,
                                  [ rdf:type owl:Restriction ;
                                    owl:onProperty <http://www.w3.org/2003/01/geo/wgs84_pos#long> ;
                                    owl:someValuesFrom xsd:float
                                  ] ;
                  rdfs:comment "The absolute poistion of an automotive object in terms of lat, long and lat"@en ;
                  rdfs:label "AbsolutePosition"@en .


###  https://saref.etsi.org/saref4auto/AbsoluteSpeed
:AbsoluteSpeed rdf:type owl:Class ;
               rdfs:subClassOf :Speed ;
               rdfs:comment "A type of speed"@en ;
               rdfs:label "AbsoluteSpeed"@en .


###  https://saref.etsi.org/saref4auto/Acceleration
:Acceleration rdf:type owl:Class ;
              rdfs:subClassOf <https://saref.etsi.org/core/Property> ;
              rdfs:comment "A Property of interest for the automotive domain"@en ;
              rdfs:label "Acceleration"@en .


###  https://saref.etsi.org/saref4auto/AccelerationConfidence
:AccelerationConfidence rdf:type owl:Class ;
                        rdfs:subClassOf :Confidence ,
                                        [ rdf:type owl:Restriction ;
                                          owl:onProperty :hasConfidenceValue ;
                                          owl:someValuesFrom xsd:float
                                        ] ;
                        rdfs:comment "A type of confidence for acceleration measurements that represents the absolute accuracy of a reported vehicle acceleration value with a predefined confidence level (e.g. 95 %)"@en ;
                        rdfs:label "AccelerationConfidence"@en .


###  https://saref.etsi.org/saref4auto/Address
:Address rdf:type owl:Class ;
         rdfs:comment "A class to define common information related to an address. It is out of scope of SAREF4AUTO to define the details of such an address. It is instead recommended to reuse existing ontologies that specify how to model an address in terms of Street, Postal Code, City, Region, Country, etc."@en ;
         rdfs:label "Address"@en .


###  https://saref.etsi.org/saref4auto/AngularDirection
:AngularDirection rdf:type owl:Class ;
                  rdfs:subClassOf :Heading ;
                  rdfs:comment "A type of heading"@en ;
                  rdfs:label "AngularDirection"@en .


###  https://saref.etsi.org/saref4auto/Assembling
:Assembling rdf:type owl:Class ;
            rdfs:subClassOf :PlatoonState ;
            rdfs:comment "A type of state for Platoon"@en ;
            rdfs:label "assembling"@en .


###  https://saref.etsi.org/saref4auto/AtDropOffSpot
:AtDropOffSpot rdf:type owl:Class ;
               rdfs:subClassOf :ParkingVehicleState ;
               rdfs:comment "A type of state for Parking Vehicle"@en ;
               rdfs:label "At Drop Off Spot"@en .


###  https://saref.etsi.org/saref4auto/AtPickUpSpot
:AtPickUpSpot rdf:type owl:Class ;
              rdfs:subClassOf :ParkingVehicleState ;
              rdfs:comment "A type of state for Parking Vehicle"@en ;
              rdfs:label "At Pick Up Spot"@en .


###  https://saref.etsi.org/saref4auto/AutomationLevel
:AutomationLevel rdf:type owl:Class ;
                 rdfs:comment "The level of automation a platoon of vehicles or a singular vehicle"@en ;
                 rdfs:label "AutomationLevel"@en .


###  https://saref.etsi.org/saref4auto/AutomotiveObject
:AutomotiveObject rdf:type owl:Class ;
                  rdfs:comment "The main objects of interest in the automotive domain."@en ;
                  rdfs:label "AutomotiveObject"@en .


###  https://saref.etsi.org/saref4auto/BrakeCapacity
:BrakeCapacity rdf:type owl:Class ;
               rdfs:subClassOf <https://saref.etsi.org/core/Property> ;
               rdfs:comment "A Property of interest for the automotive domain"@en ;
               rdfs:label "BrakeCapacity"@en .


###  https://saref.etsi.org/saref4auto/Bus
:Bus rdf:type owl:Class ;
     rdfs:subClassOf :PublicTransport ;
     rdfs:comment "A type of public transport"@en ;
     rdfs:label "Bus"@en .


###  https://saref.etsi.org/saref4auto/Car
:Car rdf:type owl:Class ;
     rdfs:subClassOf :Vehicle ;
     rdfs:comment "A type of vehicle. Example of a car is a passenger car"@en ;
     rdfs:label "Car"@en .


###  https://saref.etsi.org/saref4auto/CardinalityUnit
:CardinalityUnit rdf:type owl:Class ;
                 rdfs:subClassOf <https://saref.etsi.org/core/UnitOfMeasure> ;
                 rdfs:comment "unit of measure of size"@en ;
                 rdfs:label "cardinality unit"@en .


###  https://saref.etsi.org/saref4auto/Charging
:Charging rdf:type owl:Class ;
          rdfs:subClassOf :ParkingSpotState ,
                          :ParkingVehicleState ;
          rdfs:comment "A type of state for Parking Spot or for Parking Vehicle"@en ;
          rdfs:label "charging"@en .


###  https://saref.etsi.org/saref4auto/Closed
:Closed rdf:type owl:Class ;
        rdfs:subClassOf :ParkingSpotState ;
        rdfs:comment "A type of state for Parking Spot"@en ;
        rdfs:label "closed"@en .


###  https://saref.etsi.org/saref4auto/Confidence
:Confidence rdf:type owl:Class ;
            rdfs:subClassOf [ rdf:type owl:Restriction ;
                              owl:onProperty :hasConfidenceUnitOfMeasure ;
                              owl:someValuesFrom <https://saref.etsi.org/core/UnitOfMeasure>
                            ] ,
                            [ rdf:type owl:Restriction ;
                              owl:onProperty :hasConfidenceValue ;
                              owl:someValuesFrom xsd:float
                            ] ;
            rdfs:comment "Every measurement in the automotive domain is an estimated measurement coming from the aggregation of several measurements from different sensor or devices taken at the same time or at consecutive times very close to each other. Therefore, a confidence is always associated to each mesurement to indicate that it has not 100% accuracy."@en ;
            rdfs:label "Confidence"@en .


###  https://saref.etsi.org/saref4auto/CriticalObject
:CriticalObject rdf:type owl:Class ;
                rdfs:subClassOf owl:Thing ,
                                [ rdf:type owl:Restriction ;
                                  owl:onProperty :hasHeight ;
                                  owl:someValuesFrom :Height
                                ] ,
                                [ rdf:type owl:Restriction ;
                                  owl:onProperty :hasLength ;
                                  owl:someValuesFrom :Length
                                ] ,
                                [ rdf:type owl:Restriction ;
                                  owl:onProperty :hasMovement ;
                                  owl:someValuesFrom :Movement
                                ] ,
                                [ rdf:type owl:Restriction ;
                                  owl:onProperty :hasShape ;
                                  owl:someValuesFrom :Shape
                                ] ,
                                [ rdf:type owl:Restriction ;
                                  owl:onProperty :hasWidth ;
                                  owl:someValuesFrom :Width
                                ] ;
                rdfs:comment "A critical object located on the road. Critical objects are small object, medium object, large object"@en ;
                rdfs:label "CriticalObject"@en .


###  https://saref.etsi.org/saref4auto/Disengaging
:Disengaging rdf:type owl:Class ;
             rdfs:subClassOf :PlatoonState ,
                             :PlatoonVehicleState ;
             rdfs:comment "A type of state for Platoon or for a Vehicle in a Platoon"@en ;
             rdfs:label "disengaging"@en .


###  https://saref.etsi.org/saref4auto/DrivingToParkingSpot
:DrivingToParkingSpot rdf:type owl:Class ;
                      rdfs:subClassOf :ParkingVehicleState ;
                      rdfs:comment "A type of state for Parking Vehicle"@en ;
                      rdfs:label "Driving To Parking Spot"@en .


###  https://saref.etsi.org/saref4auto/DrivingToPickUpSpot
:DrivingToPickUpSpot rdf:type owl:Class ;
                     rdfs:subClassOf :ParkingVehicleState ;
                     rdfs:comment "A type of state for Parking Vehicle"@en ;
                     rdfs:label "Driving To Pick Up Spot"@en .


###  https://saref.etsi.org/saref4auto/ElectricChargingParkingSpot
:ElectricChargingParkingSpot rdf:type owl:Class ;
                             rdfs:subClassOf :ParkingSpot ;
                             rdfs:comment "A type pf parking spot"@en ;
                             rdfs:label "ElectricChargingParkingSpot"@en .


###  https://saref.etsi.org/saref4auto/ElectronicControlUnit
:ElectronicControlUnit rdf:type owl:Class ;
                       rdfs:subClassOf <https://saref.etsi.org/core/Device> ,
                                       <https://saref.etsi.org/saref4syst/System> ,
                                       [ rdf:type owl:Restriction ;
                                         owl:onProperty <https://saref.etsi.org/core/measuresProperty> ;
                                         owl:someValuesFrom :Acceleration
                                       ] ,
                                       [ rdf:type owl:Restriction ;
                                         owl:onProperty <https://saref.etsi.org/core/measuresProperty> ;
                                         owl:someValuesFrom :Heading
                                       ] ,
                                       [ rdf:type owl:Restriction ;
                                         owl:onProperty <https://saref.etsi.org/core/measuresProperty> ;
                                         owl:someValuesFrom :Speed
                                       ] ,
                                       [ rdf:type owl:Restriction ;
                                         owl:onProperty :detectsPosition ;
                                         owl:someValuesFrom :Position
                                       ] ,
                                       [ rdf:type owl:Restriction ;
                                         owl:onProperty :usesMeasurement ;
                                         owl:someValuesFrom <https://saref.etsi.org/core/Measurement>
                                       ] ,
                                       [ rdf:type owl:Restriction ;
                                         owl:onProperty <https://saref.etsi.org/saref4syst/subSystemOf> ;
                                         owl:someValuesFrom :Vehicle
                                       ] ;
                       rdfs:comment "An electronic control unit (ECU) is any embedded system in automotive electronics that monitors and controls one or more of the electrical systems or subsystems in a vehicle. The ECU provides measurements about relevant properties of the vehicle, such as speed, acceleration, position, etc."@en ;
                       rdfs:label "ElectronicControlUnit"@en .


###  https://saref.etsi.org/saref4auto/EndPoint
:EndPoint rdf:type owl:Class ;
          rdfs:subClassOf :Point ;
          rdfs:comment "The final destination of a vehicle or a platoon, or the final point of a route"@en ;
          rdfs:label "EndPoint"@en .


###  https://saref.etsi.org/saref4auto/Engaging
:Engaging rdf:type owl:Class ;
          rdfs:subClassOf :PlatoonVehicleState ;
          rdfs:comment "A type of state for a Vehicle in a Platoon"@en ;
          rdfs:label "engaging"@en .


###  https://saref.etsi.org/saref4auto/Forming
:Forming rdf:type owl:Class ;
         rdfs:subClassOf :PlatoonVehicleState ;
         rdfs:comment "A type of state for a Vehicle in a Platoon"@en ;
         rdfs:label "forming"@en .


###  https://saref.etsi.org/saref4auto/Free
:Free rdf:type owl:Class ;
      rdfs:subClassOf :ParkingSpotState ;
      rdfs:comment "A type of state for Parking Spot"@en ;
      rdfs:label "free"@en .


###  https://saref.etsi.org/saref4auto/Heading
:Heading rdf:type owl:Class ;
         rdfs:subClassOf <https://saref.etsi.org/core/Property> ;
         rdfs:comment "A Property of interest for the automotive domain"@en ;
         rdfs:label "Heading"@en .


###  https://saref.etsi.org/saref4auto/HeavyTruck
:HeavyTruck rdf:type owl:Class ;
            rdfs:subClassOf :Truck ;
            rdfs:comment "A type of truck"@en ;
            rdfs:label "HeavyTruck"@en .


###  https://saref.etsi.org/saref4auto/Height
:Height rdf:type owl:Class ;
        rdfs:subClassOf <https://saref.etsi.org/core/Property> ;
        rdfs:comment "A Property of interest for the automotive domain"@en ;
        rdfs:label "Height"@en .


###  https://saref.etsi.org/saref4auto/HeightUnit
:HeightUnit rdf:type owl:Class ;
            rdfs:subClassOf <https://saref.etsi.org/core/UnitOfMeasure> ;
            rdfs:comment "unit of measure of height"@en ;
            rdfs:label "height unit"@en .


###  https://saref.etsi.org/saref4auto/Identifier
:Identifier rdf:type owl:Class ;
            rdfs:subClassOf [ rdf:type owl:Restriction ;
                              owl:onProperty :hasIDValue ;
                              owl:someValuesFrom xsd:string
                            ] ;
            rdfs:comment "A class used to identify 1)  a vehicle (station) during data exchange with other devices/stations 2) a platoon during data exchange with other devices/stations, 3)  a parking spot within a parking area during data exchange with other devices/stations. In all cases, this identifier may be a pseudonym. It may change over space and/or over time."@en ;
            rdfs:label "Identifier"@en .


###  https://saref.etsi.org/saref4auto/LargeObject
:LargeObject rdf:type owl:Class ;
             rdfs:subClassOf :CriticalObject ;
             rdfs:comment "A type of Critical Object"@en ;
             rdfs:label "Large Object"@en .


###  https://saref.etsi.org/saref4auto/LateralAcceleration
:LateralAcceleration rdf:type owl:Class ;
                     rdfs:subClassOf :Acceleration ;
                     rdfs:comment "A type of acceleration"@en ;
                     rdfs:label "Lateral Acceleration"@en .


###  https://saref.etsi.org/saref4auto/Length
:Length rdf:type owl:Class ;
        rdfs:subClassOf <https://saref.etsi.org/core/Property> ;
        rdfs:comment "A Property of interest for the automotive domain"@en ,
                     "In a platoon, a property to express that a platoon has a size. This size is defined as 1) the total number of vehicles currently in the platoon (see s4auto:Size class); or 2) Length of the platoon (sum of all vehicles' length + inter-vehicle distance)"@en ;
        rdfs:label "Length"@en .


###  https://saref.etsi.org/saref4auto/LengthUnit
:LengthUnit rdf:type owl:Class ;
            rdfs:subClassOf <https://saref.etsi.org/core/UnitOfMeasure> ;
            rdfs:comment "unit of measure of lenght"@en ;
            rdfs:label "length unit"@en .


###  https://saref.etsi.org/saref4auto/LightTruck
:LightTruck rdf:type owl:Class ;
            rdfs:subClassOf :Truck ;
            rdfs:comment "A type of truck"@en ;
            rdfs:label "LightTruck"@en .


###  https://saref.etsi.org/saref4auto/LongitudinalAcceleration
:LongitudinalAcceleration rdf:type owl:Class ;
                          rdfs:subClassOf :Acceleration ;
                          rdfs:comment "A type of acceleration"@en ;
                          rdfs:label "LongitudinalAcceleration"@en .


###  https://saref.etsi.org/saref4auto/MediumObject
:MediumObject rdf:type owl:Class ;
              rdfs:subClassOf :CriticalObject ;
              rdfs:comment "A type of Critical Object"@en ;
              rdfs:label "Medium Object"@en .


###  https://saref.etsi.org/saref4auto/Movement
:Movement rdf:type owl:Class ;
          rdfs:subClassOf <https://saref.etsi.org/core/Property> ;
          rdfs:comment "A Property of interest for the automotive domain. Relevant types of movement are: Static (position only), moving in same direction (speed, acceleration), moving in reverse direction (speed acceleration), crossing (speed, acceleration, direction)"@en ;
          rdfs:label "Movement"@en .


###  https://saref.etsi.org/saref4auto/NotifiedEvent
:NotifiedEvent rdf:type owl:Class ;
               rdfs:subClassOf owl:Thing ;
               rdfs:comment "The relevant types of events are trafficCondition, accident, roadworks, impassability, adverseWeatherCondition-Adhesion, aquaplannning, hazardousLocation-SurfaceCondition, hazardousLocation-ObstacleOnTheRoad, hazardousLocation-AnimalOnTheRoad, humanPresenceOnTheRoad, wrongWayDriving, rescueAndRecoveryWorkInProgress, adverseWeatherCondition-ExtremeWeatherCondition, adverseWeatherCondition-Visibility, adverseWeatherCondition-Precipitation, slowVehicle, dangerousEndOfQueue, vehicleBreakdown, postCrash, humanProblem, stationaryVehicle, emergencyVehicleApproaching, hazardousLocation-DangerousCurve, collisionRisk, signalViolation, dangerousSituation"@en ;
               rdfs:label "NotifiedEvent"@en .


###  https://saref.etsi.org/saref4auto/Occupied
:Occupied rdf:type owl:Class ;
          rdfs:subClassOf :ParkingSpotState ;
          rdfs:comment "A type of state for Parking Spot"@en ;
          rdfs:label "occupied"@en .


###  https://saref.etsi.org/saref4auto/P1Pedestrian
:P1Pedestrian rdf:type owl:Class ;
              rdfs:subClassOf :VulnerableRoadUser ;
              rdfs:comment "VRU Profile 1 users, for example: adult, child, elderly person, pram, animal, blind person guided by a dog, rider off its bike"@en ;
              rdfs:label "P1 Pedestrian"@en .


###  https://saref.etsi.org/saref4auto/P2Bicyclist
:P2Bicyclist rdf:type owl:Class ;
             rdfs:subClassOf :VulnerableRoadUser ;
             rdfs:comment "VRU Profile 2 users, for example: user of bicycle, wheelchair, skater, scooter, Segway, or a mounted horse rider"@en ;
             rdfs:label "P2 Bicyclist"@en .


###  https://saref.etsi.org/saref4auto/P3Motorcyclist
:P3Motorcyclist rdf:type owl:Class ;
                rdfs:subClassOf :VulnerableRoadUser ;
                rdfs:comment "VRU Profile 3 users are Motorcyclists, which are equipped with engines that allow them to move on the road. It includes users (driver and passengers, e.g. children and animals) of Powered Two Wheelers (PTW) such as mopeds (motorized scooters), motorcycles or side-cars."@en ;
                rdfs:label "P3 Motorcyclist"@en .


###  https://saref.etsi.org/saref4auto/P4Animal
:P4Animal rdf:type owl:Class ;
          rdfs:subClassOf :VulnerableRoadUser ;
          rdfs:comment "VRU Profile 4 animals presenting a safety risk to other road users, for example : dogs, wild animals, horses, cows, sheep, kangaroos, etc."@en ;
          rdfs:label "P4 Animal"@en .


###  https://saref.etsi.org/saref4auto/Parked
:Parked rdf:type owl:Class ;
        rdfs:subClassOf :ParkingVehicleState ;
        rdfs:comment "A type of state for Parking Vehicle"@en ;
        rdfs:label "parked"@en .


###  https://saref.etsi.org/saref4auto/Parking
:Parking rdf:type owl:Class ;
         rdfs:subClassOf :ParkingVehicleState ;
         rdfs:comment "A type of state for Parking Vehicle"@en ;
         rdfs:label "parking"@en .


###  https://saref.etsi.org/saref4auto/ParkingSpot
:ParkingSpot rdf:type owl:Class ;
             rdfs:subClassOf <http://www.opengis.net/ont/geosparql#Feature> ,
                             [ rdf:type owl:Restriction ;
                               owl:onProperty <http://www.opengis.net/ont/geosparql#hasGeometry> ;
                               owl:someValuesFrom :ParkingSpotPoint
                             ] ,
                             [ rdf:type owl:Restriction ;
                               owl:onProperty :hasHeight ;
                               owl:someValuesFrom :Height
                             ] ,
                             [ rdf:type owl:Restriction ;
                               owl:onProperty :hasIdentifier ;
                               owl:someValuesFrom :Identifier
                             ] ,
                             [ rdf:type owl:Restriction ;
                               owl:onProperty :hasLength ;
                               owl:someValuesFrom :Length
                             ] ,
                             [ rdf:type owl:Restriction ;
                               owl:onProperty :hasOpeningTimeAvailability ;
                               owl:someValuesFrom <http://www.w3.org/2006/time#TemporalEntity>
                             ] ,
                             [ rdf:type owl:Restriction ;
                               owl:onProperty :hasWidth ;
                               owl:someValuesFrom :Width
                             ] ,
                             [ rdf:type owl:Restriction ;
                               owl:onProperty :hasParkingSpotState ;
                               owl:maxQualifiedCardinality "1"^^xsd:nonNegativeInteger ;
                               owl:onClass :ParkingSpotState
                             ] ,
                             [ rdf:type owl:Restriction ;
                               owl:onProperty :hasDescriptionName ;
                               owl:someValuesFrom xsd:string
                             ] ;
             rdfs:comment "A location that is designated for parking. A parking spot has a geometry defining the parking area boundaries and its centre point"@en ;
             rdfs:label "ParkingSpot"@en .


###  https://saref.etsi.org/saref4auto/ParkingSpotPoint
:ParkingSpotPoint rdf:type owl:Class ;
                  rdfs:subClassOf :Point ;
                  rdfs:comment "the position of aparking spot (its centre point) in terms of lat, long and alt"@en ;
                  rdfs:label "ParkingSpotPoint"@en .


###  https://saref.etsi.org/saref4auto/ParkingSpotState
:ParkingSpotState rdf:type owl:Class ;
                  rdfs:subClassOf :State ;
                  rdfs:comment "A parking spot has a state. Possible values for parking spot state are Free, occupied, reserved, closed, charging"@en ;
                  rdfs:label "ParkingSpotState"@en .


###  https://saref.etsi.org/saref4auto/ParkingVehicleState
:ParkingVehicleState rdf:type owl:Class ;
                     rdfs:subClassOf :State ;
                     rdfs:comment "A vehicle can be found at different states (or parking phases) during parking . Possible values for parking state (or parking phase) of a vehicle are: At drop-off spot, at pick-up spot, driving to parking spot, driving to pick up spot, parking, parked, charging."@en ;
                     rdfs:label "ParkingVehicleState"@en .


###  https://saref.etsi.org/saref4auto/PassengerCar
:PassengerCar rdf:type owl:Class ;
              rdfs:subClassOf :Car ;
              rdfs:comment "A type of car"@en ;
              rdfs:label "PassengerCar"@en .


###  https://saref.etsi.org/saref4auto/PerceptionState
:PerceptionState rdf:type owl:Class ;
                 rdfs:subClassOf :State ;
                 rdfs:comment "A state of the vehicle related to its environment"@en ;
                 rdfs:label "perception state"@en .


###  https://saref.etsi.org/saref4auto/PersonalDevice
:PersonalDevice rdf:type owl:Class ;
                rdfs:subClassOf <https://saref.etsi.org/core/Device> ,
                                :AutomotiveObject ;
                rdfs:comment "A personal device is a nomadic device used by a pedestrian or the rider of a two-wheeler. A personal device in modelled as a different type of automotive object, as it normally does not have access to the vehicle CAN bus."@en ;
                rdfs:label "PersonalDevice"@en .


###  https://saref.etsi.org/saref4auto/Platoon
:Platoon rdf:type owl:Class ;
         rdfs:subClassOf [ rdf:type owl:Restriction ;
                           owl:onProperty :hasDestinationEndPoint ;
                           owl:someValuesFrom :EndPoint
                         ] ,
                         [ rdf:type owl:Restriction ;
                           owl:onProperty :hasIdentifier ;
                           owl:someValuesFrom :Identifier
                         ] ,
                         [ rdf:type owl:Restriction ;
                           owl:onProperty :hasLength ;
                           owl:someValuesFrom :Length
                         ] ,
                         [ rdf:type owl:Restriction ;
                           owl:onProperty :hasPlatoonMember ;
                           owl:someValuesFrom :Vehicle
                         ] ,
                         [ rdf:type owl:Restriction ;
                           owl:onProperty :hasPlatoonState ;
                           owl:someValuesFrom :PlatoonState
                         ] ,
                         [ rdf:type owl:Restriction ;
                           owl:onProperty :hasRoute ;
                           owl:someValuesFrom :Route
                         ] ,
                         [ rdf:type owl:Restriction ;
                           owl:onProperty :hasSize ;
                           owl:someValuesFrom :Size
                         ] ,
                         [ rdf:type owl:Restriction ;
                           owl:onProperty :hasMaxSize ;
                           owl:someValuesFrom xsd:int
                         ] ;
         rdfs:comment "A group of vehicles automatically following each other at a relatively close distance" ;
         rdfs:label "Platoon"@en .


###  https://saref.etsi.org/saref4auto/PlatoonAutomationLevel
:PlatoonAutomationLevel rdf:type owl:Class ;
                        rdfs:subClassOf :AutomationLevel ;
                        rdfs:comment "A level of automation is defined for a vehicle that it is platooning. For example, in the ENSEMBLE project  there are three levels of platoon automation defined: Level A, Level B, Level C. Level C represents the highest level of automation for platooning in terms of longitudinal and lateral control, shortest time gap supported, wider range of situations handled and support for merging of entire platoons."@en ;
                        rdfs:label "PlatoonAutomationLevel"@en .


###  https://saref.etsi.org/saref4auto/PlatoonPosition
:PlatoonPosition rdf:type owl:Class ;
                 rdfs:subClassOf :Position ,
                                 [ rdf:type owl:Restriction ;
                                   owl:onProperty :hasPlatoonIndex ;
                                   owl:someValuesFrom xsd:int
                                 ] ;
                 rdfs:comment "A vehicle member of a platoon has a platoon position that is defined as the index of the vehicle in the platoon starting from zero (leader) up to N (trailing vehicle)."@en ;
                 rdfs:label "PlatoonPosition"@en .


###  https://saref.etsi.org/saref4auto/PlatoonRole
:PlatoonRole rdf:type owl:Class ;
             rdfs:subClassOf :Role ;
             rdfs:comment "In platoon a vehicle can assume roles such as: unknown, leader, follower, ready-for-leading, trailing, etc."@en ;
             rdfs:label "PlatoonRole"@en .


###  https://saref.etsi.org/saref4auto/PlatoonState
:PlatoonState rdf:type owl:Class ;
              rdfs:subClassOf :State ;
              rdfs:comment "The state of a platoon. Examples of states for a platoon are: unknown, standalone, assembling, platooning, disengaging, etc."@en ;
              rdfs:label "PlatoonState"@en .


###  https://saref.etsi.org/saref4auto/PlatoonVehicleState
:PlatoonVehicleState rdf:type owl:Class ;
                     rdfs:subClassOf :State ;
                     rdfs:comment "Examples of states for a vehicle in a platoon are: unknown, standalone, engaging, platooning, disengaging, searching, forming."@en ;
                     rdfs:label "PlatoonVehicleState"@en .


###  https://saref.etsi.org/saref4auto/Platooning
:Platooning rdf:type owl:Class ;
            rdfs:subClassOf :PlatoonState ,
                            :PlatoonVehicleState ;
            rdfs:comment "A type of state for Platoon or for a Vehicle in a Platoon"@en ;
            rdfs:label "platooning"@en .


###  https://saref.etsi.org/saref4auto/Point
:Point rdf:type owl:Class ;
       rdfs:subClassOf <http://www.opengis.net/ont/geosparql#Geometry> ,
                       <http://www.w3.org/2003/01/geo/wgs84_pos#Point> ;
       rdfs:comment "A geo point in SAREF4AUTO"@en ;
       rdfs:label "Point"@en .


###  https://saref.etsi.org/saref4auto/Position
:Position rdf:type owl:Class ;
          rdfs:subClassOf [ rdf:type owl:Restriction ;
                            owl:onProperty :hasConfidence ;
                            owl:someValuesFrom :Confidence
                          ] ;
          rdfs:comment "The position of an entity in the automotive domain"@en ;
          rdfs:label "Position"@en .


###  https://saref.etsi.org/saref4auto/PositionConfidenceEllipse
:PositionConfidenceEllipse rdf:type owl:Class ;
                           rdfs:subClassOf :Confidence ;
                           rdfs:comment "A type of confidence that represents horizontal position accuracy in a shape of ellipse with a predefined confidence level (e.g. 95 %). The centre of the ellipse shape corresponds to the reference position point for which the position accuracy is evaluated."@en ;
                           rdfs:label "PositionConfidenceEllipse"@en .


###  https://saref.etsi.org/saref4auto/PublicTransport
:PublicTransport rdf:type owl:Class ;
                 rdfs:subClassOf :Vehicle .


###  https://saref.etsi.org/saref4auto/RegularParkingSpot
:RegularParkingSpot rdf:type owl:Class ;
                    rdfs:subClassOf :ParkingSpot ;
                    rdfs:comment "A type pf parking spot"@en ;
                    rdfs:label "RegularParkingSpot"@en .


###  https://saref.etsi.org/saref4auto/RelativePosition
:RelativePosition rdf:type owl:Class ;
                  rdfs:subClassOf :Position ,
                                  [ rdf:type owl:Restriction ;
                                    owl:onProperty :hasCoordinateX ;
                                    owl:someValuesFrom xsd:float
                                  ] ,
                                  [ rdf:type owl:Restriction ;
                                    owl:onProperty :hasCoordinateY ;
                                    owl:someValuesFrom xsd:float
                                  ] ,
                                  [ rdf:type owl:Restriction ;
                                    owl:onProperty :hasCoordinateZ ;
                                    owl:someValuesFrom xsd:float
                                  ] ;
                  rdfs:comment "It represents the relative position of a vehicle (e.g., a car is x,y,z in front of another car)"@en ;
                  rdfs:label "RelativePosition"@en .


###  https://saref.etsi.org/saref4auto/RelativeSpeed
:RelativeSpeed rdf:type owl:Class ;
               rdfs:subClassOf :Speed ;
               rdfs:comment "A type of speed"@en ;
               rdfs:label "RelativeSpeed"@en .


###  https://saref.etsi.org/saref4auto/RendezvousLocation
:RendezvousLocation rdf:type owl:Class ;
                    rdfs:subClassOf :Point ;
                    rdfs:comment "It is the estimated location where the vehicle member joins the platoon. It is expressed in global coordinates (lat, long, alt), e.g. according to WGS 84."@en ;
                    rdfs:label "RendezvousLocation"@en .


###  https://saref.etsi.org/saref4auto/Reserved
:Reserved rdf:type owl:Class ;
          rdfs:subClassOf :ParkingSpotState ;
          rdfs:comment "A type of state for Parking Spot"@en ;
          rdfs:label "reserved"@en .


###  https://saref.etsi.org/saref4auto/RoadEntity
:RoadEntity rdf:type owl:Class ;
            rdfs:subClassOf <https://saref.etsi.org/core/FeatureOfInterest> ,
                            [ rdf:type owl:Restriction ;
                              owl:onProperty :consistsOfEquipment ;
                              owl:someValuesFrom :RoadSideEquipment
                            ] ,
                            [ rdf:type owl:Restriction ;
                              owl:onProperty :consistsOfEvent ;
                              owl:someValuesFrom :NotifiedEvent
                            ] ,
                            [ rdf:type owl:Restriction ;
                              owl:onProperty :consistsOfObject ;
                              owl:someValuesFrom :CriticalObject
                            ] ,
                            [ rdf:type owl:Restriction ;
                              owl:onProperty :consistsOfUser ;
                              owl:someValuesFrom :VulnerableRoadUser
                            ] ,
                            [ rdf:type owl:Restriction ;
                              owl:onProperty :hasAbsolutePosition ;
                              owl:someValuesFrom :AbsolutePosition
                            ] ,
                            [ rdf:type owl:Restriction ;
                              owl:onProperty :hasHeight ;
                              owl:someValuesFrom :Height
                            ] ,
                            [ rdf:type owl:Restriction ;
                              owl:onProperty :hasLength ;
                              owl:someValuesFrom :Length
                            ] ,
                            [ rdf:type owl:Restriction ;
                              owl:onProperty :hasMovement ;
                              owl:someValuesFrom :Movement
                            ] ,
                            [ rdf:type owl:Restriction ;
                              owl:onProperty :hasRelativePosition ;
                              owl:someValuesFrom :RelativePosition
                            ] ,
                            [ rdf:type owl:Restriction ;
                              owl:onProperty :hasShape ;
                              owl:someValuesFrom :Shape
                            ] ,
                            [ rdf:type owl:Restriction ;
                              owl:onProperty :hasWidth ;
                              owl:someValuesFrom :Width
                            ] ;
            rdfs:comment "An entity present on the road in the neighbouring area of a vehicle"@en ;
            rdfs:label "RoadEntity"@en .


###  https://saref.etsi.org/saref4auto/RoadObject
:RoadObject rdf:type owl:Class ;
            rdfs:subClassOf <https://saref.etsi.org/core/FeatureOfInterest> ;
            rdfs:comment "Road side sensors measure properties (such as speed, position, dimension, direction, etc.) of road objects. Types of relevant road objects are Pedestrian, vehicles, obstacles, traffic signs, etc."@en ;
            rdfs:label "RoadObject"@en .


###  https://saref.etsi.org/saref4auto/RoadSideActuator
:RoadSideActuator rdf:type owl:Class ;
                  rdfs:subClassOf <https://saref.etsi.org/core/Actuator> ,
                                  [ rdf:type owl:Restriction ;
                                    owl:onProperty :usesMeasurement ;
                                    owl:someValuesFrom <https://saref.etsi.org/core/Measurement>
                                  ] ;
                  rdfs:comment "Devices deployed along the road that produce signals based on road side sensor data measurements. Types of road side actuators that are relevant are devices such as traffic light controllers changing from red to green based on detected vehicles."@en ;
                  rdfs:label """RoadSideActuator
"""@en .


###  https://saref.etsi.org/saref4auto/RoadSideEquipment
:RoadSideEquipment rdf:type owl:Class ;
                   rdfs:subClassOf :AutomotiveObject ;
                   rdfs:comment "A road side equipment can be either a simple data relay between vehicles and infrastructure or between the vehicles themselves, or it can run applications. It is usually high mounted in existing equipment, such as a street light, city traffic light, VMS or highway sign, or has its own pole."@en ;
                   rdfs:label "RoadSideEquipment"@en .


###  https://saref.etsi.org/saref4auto/RoadSideSensor
:RoadSideSensor rdf:type owl:Class ;
                rdfs:subClassOf <https://saref.etsi.org/core/Sensor> ,
                                [ rdf:type owl:Restriction ;
                                  owl:onProperty <https://saref.etsi.org/core/measuresProperty> ;
                                  owl:someValuesFrom :Heading
                                ] ,
                                [ rdf:type owl:Restriction ;
                                  owl:onProperty <https://saref.etsi.org/core/measuresProperty> ;
                                  owl:someValuesFrom :Height
                                ] ,
                                [ rdf:type owl:Restriction ;
                                  owl:onProperty <https://saref.etsi.org/core/measuresProperty> ;
                                  owl:someValuesFrom :Length
                                ] ,
                                [ rdf:type owl:Restriction ;
                                  owl:onProperty <https://saref.etsi.org/core/measuresProperty> ;
                                  owl:someValuesFrom :Speed
                                ] ,
                                [ rdf:type owl:Restriction ;
                                  owl:onProperty <https://saref.etsi.org/core/measuresProperty> ;
                                  owl:someValuesFrom :Width
                                ] ,
                                [ rdf:type owl:Restriction ;
                                  owl:onProperty :detectsPosition ;
                                  owl:someValuesFrom :AbsolutePosition
                                ] ,
                                [ rdf:type owl:Restriction ;
                                  owl:onProperty :detectsPosition ;
                                  owl:someValuesFrom :RelativePosition
                                ] ;
                rdfs:comment "Sensors such as cameras, radars that are deployed along the road (e.g. at intersections and at poles along a highway). Road side sensors perform measurements, such as speed, position (relative or absolute), dimension, direction, etc. of road objects."@en ;
                rdfs:label "RoadSideSensor"@en .


###  https://saref.etsi.org/saref4auto/RoadTopologyPosition
:RoadTopologyPosition rdf:type owl:Class ;
                      rdfs:subClassOf :Position ;
                      rdfs:comment "Position with respect to road topology (e.g. road, segment or lane) and lane characteristics (highway lane, road lane, bicycle lane, pavement, off-road)."@en ;
                      rdfs:label "Road Topology Position"@en .


###  https://saref.etsi.org/saref4auto/Role
:Role rdf:type owl:Class ;
      rdfs:comment "The role that can be assumed by a vehicle or a platoon"@en ;
      rdfs:label "Role"@en .


###  https://saref.etsi.org/saref4auto/Route
:Route rdf:type owl:Class ;
       rdfs:subClassOf [ rdf:type owl:Restriction ;
                         owl:onProperty :hasDestinationEndPoint ;
                         owl:someValuesFrom :EndPoint
                       ] ,
                       [ rdf:type owl:Restriction ;
                         owl:onProperty :hasOrigin ;
                         owl:someValuesFrom :StartPoint
                       ] ,
                       [ rdf:type owl:Restriction ;
                         owl:onProperty :isCollectionOf ;
                         owl:someValuesFrom :RoutePoint
                       ] ;
       rdfs:comment "The route of a vehicle or of a platoon. The route of a platoon is defined as the route of the current vehicle leader in the platoon that other follower vehicles (partially) share"@en ;
       rdfs:label "Route"@en .


###  https://saref.etsi.org/saref4auto/RoutePoint
:RoutePoint rdf:type owl:Class ;
            rdfs:subClassOf :Point ;
            rdfs:comment "The intermediate points of a route"@en ;
            rdfs:label "RoutePoint"@en .


###  https://saref.etsi.org/saref4auto/Searching
:Searching rdf:type owl:Class ;
           rdfs:subClassOf :PlatoonVehicleState ;
           rdfs:comment "A type of state for a Vehicle in a Platoon"@en ;
           rdfs:label "Searching"@en .


###  https://saref.etsi.org/saref4auto/Shape
:Shape rdf:type owl:Class ;
       rdfs:subClassOf <https://saref.etsi.org/core/Property> ;
       rdfs:comment "A Property of interest for the automotive domain. It defines the overall shape of an entity: i.e., Sphere, Torus, Cylinder, Cone, Ellipsoid, Cube, Cuboid, Pyramid, Prism, Multiple shapes"@en ;
       rdfs:label "Shape"@en .


###  https://saref.etsi.org/saref4auto/Size
:Size rdf:type owl:Class ;
      rdfs:subClassOf <https://saref.etsi.org/core/Property> ;
      rdfs:comment "A Property of interest for the automotive domain. A platoon has a size. Tis size is defined as 1) the total number of vehicles currently in the platoon; or 2) Length of the platoon (sum of all vehicles' length + inter-vehicle distance)"@en ;
      rdfs:label "Size"@en .


###  https://saref.etsi.org/saref4auto/SmallObject
:SmallObject rdf:type owl:Class ;
             rdfs:subClassOf :CriticalObject ;
             rdfs:comment "A type of Critical Object"@en ;
             rdfs:label "Small Object"@en .


###  https://saref.etsi.org/saref4auto/SpecialPermitParkingSpot
:SpecialPermitParkingSpot rdf:type owl:Class ;
                          rdfs:subClassOf :ParkingSpot ;
                          rdfs:comment "A type pf parking spot. Parking spot reserved for special permits (authorities, disabled, blue Zone, resident ...)"@en ;
                          rdfs:label "SpecialPermitParkingSpot"@en .


###  https://saref.etsi.org/saref4auto/Speed
:Speed rdf:type owl:Class ;
       rdfs:subClassOf <https://saref.etsi.org/core/Property> ;
       rdfs:comment "A Property of interest for the automotive domain"@en ;
       rdfs:label "Speed"@en .


###  https://saref.etsi.org/saref4auto/SpeedConfidence
:SpeedConfidence rdf:type owl:Class ;
                 rdfs:subClassOf :Confidence ,
                                 [ rdf:type owl:Restriction ;
                                   owl:onProperty :hasConfidenceValue ;
                                   owl:someValuesFrom xsd:int
                                 ] ;
                 rdfs:comment "A type of confidence for speed measurements that represents absolute accuracy of a speed value in cm/s"@en ;
                 rdfs:label "SpeedConfidence"@en .


###  https://saref.etsi.org/saref4auto/SpeedUnit
:SpeedUnit rdf:type owl:Class ;
           rdfs:subClassOf <https://saref.etsi.org/core/UnitOfMeasure> ;
           rdfs:comment "unit of measure of speed"@en ;
           rdfs:label "speed unit"@en .


###  https://saref.etsi.org/saref4auto/Standalone
:Standalone rdf:type owl:Class ;
            rdfs:subClassOf :PlatoonState ,
                            :PlatoonVehicleState ;
            rdfs:comment "A type of state for Platoon or for a Vehicle in a Platoon"@en ;
            rdfs:label "standalone"@en .


###  https://saref.etsi.org/saref4auto/StartPoint
:StartPoint rdf:type owl:Class ;
            rdfs:subClassOf :Point ;
            rdfs:comment "The origin of a route"@en ;
            rdfs:label "StartPoint"@en .


###  https://saref.etsi.org/saref4auto/State
:State rdf:type owl:Class ;
       rdfs:subClassOf <https://saref.etsi.org/core/State> ,
                       [ rdf:type owl:Restriction ;
                         owl:onProperty <https://saref.etsi.org/core/hasTimestamp> ;
                         owl:someValuesFrom xsd:dateTime
                       ] ;
       rdfs:comment "A class dedicated to describe the relevant states in the automotive domain"@en ;
       rdfs:label "State"@en .


###  https://saref.etsi.org/saref4auto/StationID
:StationID rdf:type owl:Class ;
           rdfs:subClassOf :Identifier ;
           rdfs:comment "A type of identifier for vehicles and platoons, as defined in ETSI TS 102 894-2."@en ;
           rdfs:label "StationID"@en .


###  https://saref.etsi.org/saref4auto/TrafficLightController
:TrafficLightController rdf:type owl:Class ;
                        rdfs:subClassOf :RoadSideActuator ;
                        rdfs:comment "A device that automatically operates coloured lights, typically red, amber, and green, for controlling traffic at road junctions, pedestrian crossings, and roundabouts."@en ;
                        rdfs:label "TrafficLight"@en .


###  https://saref.etsi.org/saref4auto/TrafficManagementCentre
:TrafficManagementCentre rdf:type owl:Class ;
                         rdfs:subClassOf :AutomotiveObject ;
                         rdfs:comment "A traffic centre provides services to road users: exploiting data for road traffic management, providing information about mobility zones, operational management of the road infrastructure, etc."@en ;
                         rdfs:label "TrafficManagementCentre"@en .


###  https://saref.etsi.org/saref4auto/Tram
:Tram rdf:type owl:Class ;
      rdfs:subClassOf :PublicTransport ;
      rdfs:comment "A type of public transport"@en ;
      rdfs:label "tram"@en .


###  https://saref.etsi.org/saref4auto/Truck
:Truck rdf:type owl:Class ;
       rdfs:subClassOf :Vehicle ;
       rdfs:comment "A type of vehicle. Example of trucks are heavy trucks or light trucks."@en ;
       rdfs:label "Truck"@en .


###  https://saref.etsi.org/saref4auto/TwoWheeler
:TwoWheeler rdf:type owl:Class ;
            rdfs:subClassOf :Vehicle ;
            rdfs:comment "A type of vehicle. This class involves all sorts of two wheelers, from motorcycles to bicycles and (e-)scooters."@en ;
            rdfs:label "TwoWheeler"@en .


###  https://saref.etsi.org/saref4auto/UUID
:UUID rdf:type owl:Class ;
      rdfs:subClassOf :Identifier ;
      rdfs:comment "A universally unique identifier (UUID) is a 128-bit number used to identify items and is also known as: globally unique identifier (GUID). In its canonical textual representation, the sixteen octets of a UUID are represented as 32 hexadecimal (base 16) digits, displayed in five groups separated by hyphens, in the form 8-4-4-4-12 for a total of 36 characters (32 alphanumeric characters and four hyphens). UUID are documented in ISO/IEC 11578:1996 \"Information technology – Open Systems Interconnection – Remote Procedure Call (RPC)\" and in ITU-T Rec. X.667 ISO/IEC 9834-8:2005."@en ;
      rdfs:label "UUID"@en .


###  https://saref.etsi.org/saref4auto/Unknown
:Unknown rdf:type owl:Class ;
         rdfs:subClassOf :PlatoonState ,
                         :PlatoonVehicleState .


###  https://saref.etsi.org/saref4auto/Vehicle
:Vehicle rdf:type owl:Class ;
         rdfs:subClassOf <https://saref.etsi.org/core/FeatureOfInterest> ,
                         :AutomotiveObject ,
                         <https://saref.etsi.org/saref4syst/System> ,
                         [ rdf:type owl:Restriction ;
                           owl:onProperty :hasAbsolutePosition ;
                           owl:someValuesFrom :AbsolutePosition
                         ] ,
                         [ rdf:type owl:Restriction ;
                           owl:onProperty :hasAutomationLevel ;
                           owl:someValuesFrom :AutomationLevel
                         ] ,
                         [ rdf:type owl:Restriction ;
                           owl:onProperty :hasBrakeCapacity ;
                           owl:someValuesFrom :BrakeCapacity
                         ] ,
                         [ rdf:type owl:Restriction ;
                           owl:onProperty :hasDestinationAddress ;
                           owl:someValuesFrom :Address
                         ] ,
                         [ rdf:type owl:Restriction ;
                           owl:onProperty :hasDestinationEndPoint ;
                           owl:someValuesFrom :EndPoint
                         ] ,
                         [ rdf:type owl:Restriction ;
                           owl:onProperty :hasEnvironment ;
                           owl:someValuesFrom :VehicleEnvironment
                         ] ,
                         [ rdf:type owl:Restriction ;
                           owl:onProperty :hasEstimatedRendezvousLocation ;
                           owl:someValuesFrom :RendezvousLocation
                         ] ,
                         [ rdf:type owl:Restriction ;
                           owl:onProperty :hasHeight ;
                           owl:someValuesFrom :Height
                         ] ,
                         [ rdf:type owl:Restriction ;
                           owl:onProperty :hasIdentifier ;
                           owl:someValuesFrom :Identifier
                         ] ,
                         [ rdf:type owl:Restriction ;
                           owl:onProperty :hasLength ;
                           owl:someValuesFrom :Length
                         ] ,
                         [ rdf:type owl:Restriction ;
                           owl:onProperty :hasParkingVehicleState ;
                           owl:someValuesFrom :PlatoonVehicleState
                         ] ,
                         [ rdf:type owl:Restriction ;
                           owl:onProperty :hasPlatoonPosition ;
                           owl:someValuesFrom :PlatoonPosition
                         ] ,
                         [ rdf:type owl:Restriction ;
                           owl:onProperty :hasPlatoonRole ;
                           owl:someValuesFrom :PlatoonRole
                         ] ,
                         [ rdf:type owl:Restriction ;
                           owl:onProperty :hasPlatoonVehicleState ;
                           owl:someValuesFrom :PlatoonVehicleState
                         ] ,
                         [ rdf:type owl:Restriction ;
                           owl:onProperty :hasRelativePosition ;
                           owl:someValuesFrom :RelativePosition
                         ] ,
                         [ rdf:type owl:Restriction ;
                           owl:onProperty :hasRoadTopologyPosition ;
                           owl:someValuesFrom :RoadTopologyPosition
                         ] ,
                         [ rdf:type owl:Restriction ;
                           owl:onProperty :hasRoute ;
                           owl:someValuesFrom :Route
                         ] ,
                         [ rdf:type owl:Restriction ;
                           owl:onProperty :hasVehicleRole ;
                           owl:someValuesFrom :VehicleRole
                         ] ,
                         [ rdf:type owl:Restriction ;
                           owl:onProperty :hasWidth ;
                           owl:someValuesFrom :Width
                         ] ,
                         [ rdf:type owl:Restriction ;
                           owl:onProperty :isMemberOfPlatoon ;
                           owl:someValuesFrom :Platoon
                         ] ,
                         [ rdf:type owl:Restriction ;
                           owl:onProperty :isMemberOfVehicleEnvironment ;
                           owl:someValuesFrom :VehicleEnvironment
                         ] ,
                         [ rdf:type owl:Restriction ;
                           owl:onProperty <https://saref.etsi.org/saref4syst/hasSubSystem> ;
                           owl:someValuesFrom :ElectronicControlUnit
                         ] ,
                         [ rdf:type owl:Restriction ;
                           owl:onProperty :hasEstimatedJoiningTime ;
                           owl:someValuesFrom xsd:dateTime
                         ] ;
         rdfs:comment "A vehicle is the main object of interest in the automotive domain. Example of types of vehicles are car, truck, public transport and two-wheeler. See ETSI TS 102 894-2 spec for full list of vehicles, which are type of \"stations\". See also the SENSORIS data model for possible type of vehicles. The main IoT device considered in the vehicle is the ECU (part of the vehicle on board equipment, or OBE), see s4auto:ElectronicControlUnit class."@en ;
         rdfs:label "Vehicle"@en .


###  https://saref.etsi.org/saref4auto/VehicleAutomationLevel
:VehicleAutomationLevel rdf:type owl:Class ;
                        rdfs:subClassOf :AutomationLevel ;
                        rdfs:comment """According to SAE J3016, there are five levels of automation for a vehicle:
- Level 0: No Driving Automation.
- Level 1: Driver assistance.
- Level 2: Partial driving automation.
- Level 3: Conditional driving automation.
- Level 4: High driving automation.
- Level 5: Full Driving automation."""@en ;
                        rdfs:label "VehicleAutomationLevel"@en .


###  https://saref.etsi.org/saref4auto/VehicleEnvironment
:VehicleEnvironment rdf:type owl:Class ;
                    rdfs:subClassOf [ rdf:type owl:Restriction ;
                                      owl:onProperty :consistsOfEntity ;
                                      owl:someValuesFrom :RoadEntity
                                    ] ,
                                    [ rdf:type owl:Restriction ;
                                      owl:onProperty :consistsOfVehicle ;
                                      owl:someValuesFrom :Vehicle
                                    ] ;
                    rdfs:comment "The vehicle environment is made of entities which are present on the road in the area around the vehicle"@en ;
                    rdfs:label "VehicleEnvironment"@en .


###  https://saref.etsi.org/saref4auto/VehicleRole
:VehicleRole rdf:type owl:Class ;
             rdfs:subClassOf :Role ;
             rdfs:comment "The role the vehicle plays in traffic. If not specified, it is assumed that it takes a default value. Otherwise, possible values to be specified are: publicTransport, specialTransport, dangerousGoods, roadWork, rescue, emergency, safetyCar, agriculture, commercial, military, roadOperator, taxi."@en ;
             rdfs:label "VehicleRole"@en .


###  https://saref.etsi.org/saref4auto/VulnerableRoadUser
:VulnerableRoadUser rdf:type owl:Class ;
                    rdfs:subClassOf owl:Thing ,
                                    [ rdf:type owl:Restriction ;
                                      owl:onProperty :hasHeight ;
                                      owl:someValuesFrom :Height
                                    ] ,
                                    [ rdf:type owl:Restriction ;
                                      owl:onProperty :hasLength ;
                                      owl:someValuesFrom :Length
                                    ] ,
                                    [ rdf:type owl:Restriction ;
                                      owl:onProperty :hasMovement ;
                                      owl:someValuesFrom :Movement
                                    ] ,
                                    [ rdf:type owl:Restriction ;
                                      owl:onProperty :hasWidth ;
                                      owl:someValuesFrom :Width
                                    ] ;
                    rdfs:comment "Non-motorized road users as well as users of VRU vehicles (L class of vehicles, for example mopeds or motorcycles, etc.) participating to the road traffic" ;
                    rdfs:label "VulnerableRoadUser"@en .


###  https://saref.etsi.org/saref4auto/Weight
:Weight rdf:type owl:Class ;
        rdfs:subClassOf <https://saref.etsi.org/core/Property> ;
        rdfs:comment "A Property of interest for the automotive domain"@en ;
        rdfs:label "Weight"@en .


###  https://saref.etsi.org/saref4auto/Width
:Width rdf:type owl:Class ;
       rdfs:subClassOf <https://saref.etsi.org/core/Property> ;
       rdfs:comment "A Property of interest for the automotive domain"@en ;
       rdfs:label "Width"@en .


###  https://saref.etsi.org/saref4auto/WidthUnit
:WidthUnit rdf:type owl:Class ;
           rdfs:subClassOf <https://saref.etsi.org/core/UnitOfMeasure> ;
           rdfs:comment "unit of measure of width"@en ;
           rdfs:label "width unit"@en .


###  https://saref.etsi.org/saref4auto/YawRate
:YawRate rdf:type owl:Class ;
         rdfs:subClassOf :Heading ;
         rdfs:comment "A type of heading"@en ;
         rdfs:label "YawRate"@en .


###  https://saref.etsi.org/saref4syst/System
<https://saref.etsi.org/saref4syst/System> rdf:type owl:Class ;
                                           rdfs:comment "The class of systems, i.e., systems virtually isolated from the environment, whose behaviour and interactions with the environment are modeled. Systems can be connected to other systems. Connected systems interact in some ways. Systems can also have subsystems. Properties of subsystems somehow contribute to the properties of the supersystem"@en ;
                                           rdfs:isDefinedBy <https://saref.etsi.org/saref4syst/> ;
                                           rdfs:label "System"@en .


#################################################################
#    Individuals
#################################################################

###  https://saref.etsi.org/saref4auto/Agriculture
:Agriculture rdf:type owl:NamedIndividual ,
                      :VehicleRole ;
             rdfs:comment "A type of vehicle role"@en ;
             rdfs:label "agriculture"@en .


###  https://saref.etsi.org/saref4auto/Commercial
:Commercial rdf:type owl:NamedIndividual ,
                     :VehicleRole ;
            rdfs:comment "A type of vehicle role"@en ;
            rdfs:label "commercial"@en .


###  https://saref.etsi.org/saref4auto/CrossingLeft
:CrossingLeft rdf:type owl:NamedIndividual ,
                       :Movement ;
              rdfs:comment "A type of movement"@en ;
              rdfs:label "crossing Left"@en .


###  https://saref.etsi.org/saref4auto/CrossingRight
:CrossingRight rdf:type owl:NamedIndividual ,
                        :Movement ;
               rdfs:comment "A type of movement"@en ;
               rdfs:label "crossing Right"@en .


###  https://saref.etsi.org/saref4auto/DangerousGood
:DangerousGood rdf:type owl:NamedIndividual ,
                        :VehicleRole ;
               rdfs:comment "A type of vehicle role"@en ;
               rdfs:label "dangerousGoods"@en .


###  https://saref.etsi.org/saref4auto/Emergency
:Emergency rdf:type owl:NamedIndividual ,
                    :VehicleRole ;
           rdfs:comment "A type of vehicle role"@en ;
           rdfs:label "emergency"@en .


###  https://saref.etsi.org/saref4auto/Follower
:Follower rdf:type owl:NamedIndividual ,
                   :PlatoonRole ;
          rdfs:comment "A type of platoon role"@en ;
          rdfs:label "follower"@en .


###  https://saref.etsi.org/saref4auto/Leader
:Leader rdf:type owl:NamedIndividual ,
                 :PlatoonRole ;
        rdfs:comment "A type of platoon role"@en ;
        rdfs:label "leader"@en .


###  https://saref.etsi.org/saref4auto/Military
:Military rdf:type owl:NamedIndividual ,
                   :VehicleRole ;
          rdfs:comment "A type of vehicle role"@en ;
          rdfs:label "military"@en .


###  https://saref.etsi.org/saref4auto/PublicTransport
:PublicTransport rdf:type owl:NamedIndividual ,
                          :VehicleRole .


###  https://saref.etsi.org/saref4auto/ReadyForLeading
:ReadyForLeading rdf:type owl:NamedIndividual ,
                          :PlatoonRole ;
                 rdfs:comment "A type of platoon role"@en ;
                 rdfs:label "ready for leading"@en .


###  https://saref.etsi.org/saref4auto/Rescue
:Rescue rdf:type owl:NamedIndividual ,
                 :VehicleRole ;
        rdfs:comment "A type of vehicle role"@en ;
        rdfs:label "rescue"@en .


###  https://saref.etsi.org/saref4auto/ReverseDirection
:ReverseDirection rdf:type owl:NamedIndividual ,
                           :Movement ;
                  rdfs:comment "A type of movement"@en ;
                  rdfs:label "reverse Direction"@en .


###  https://saref.etsi.org/saref4auto/RoadOperator
:RoadOperator rdf:type owl:NamedIndividual ,
                       :VehicleRole ;
              rdfs:comment "A type of vehicle role"@en ;
              rdfs:label "roadOperator"@en .


###  https://saref.etsi.org/saref4auto/RoadWork
:RoadWork rdf:type owl:NamedIndividual ,
                   :VehicleRole ;
          rdfs:comment "A type of vehicle role"@en ;
          rdfs:label "roadWork"@en .


###  https://saref.etsi.org/saref4auto/SafetyCar
:SafetyCar rdf:type owl:NamedIndividual ,
                    :VehicleRole ;
           rdfs:comment "A type of vehicle role"@en ;
           rdfs:label "safetyCar"@en .


###  https://saref.etsi.org/saref4auto/SameDirection
:SameDirection rdf:type owl:NamedIndividual ,
                        :Movement ;
               rdfs:comment "A type of movement"@en ;
               rdfs:label "same Direction"@en .


###  https://saref.etsi.org/saref4auto/SpecialTransport
:SpecialTransport rdf:type owl:NamedIndividual ,
                           :VehicleRole ;
                  rdfs:comment "A type of vehicle role"@en ;
                  rdfs:label "specialTransport"@en .


###  https://saref.etsi.org/saref4auto/Static
:Static rdf:type owl:NamedIndividual ,
                 :Movement ;
        rdfs:comment "A type of movement"@en ;
        rdfs:label "static"@en .


###  https://saref.etsi.org/saref4auto/Taxi
:Taxi rdf:type owl:NamedIndividual ,
               :VehicleRole ;
      rdfs:comment "A type of vehicle role"@en ;
      rdfs:label "taxi"@en .


###  https://saref.etsi.org/saref4auto/Trailing
:Trailing rdf:type owl:NamedIndividual ,
                   :PlatoonRole ;
          rdfs:comment "A type of platoon role"@en ;
          rdfs:label "trailing"@en .


###  https://saref.etsi.org/saref4auto/Unknown
:Unknown rdf:type owl:NamedIndividual ,
                  :PlatoonRole .


#################################################################
#    Annotations
#################################################################

:PublicTransport rdfs:comment "A type of vehicle role"@en ,
                              "A type of vehicle. Example of public transport is a bus or a tram"@en ;
                 rdfs:label "PublicTransport"@en ,
                            "publicTransport"@en .


:Unknown rdfs:comment "A type of platoon role"@en ,
                      "A type of state for Platoon or for a Vehicle in a Platoon"@en ;
         rdfs:label "unknown"@en .


###  Generated by the OWL API (version 5.1.14) https://github.com/owlcs/owlapi/
